Checkpoint.

src/coq/Semantics/InfiniteToFinite.v
@@ -332,13 +332,15 @@ Module InfiniteToFinite.
     - exact (lift_local_env a :: IHstack).
   Defined.
 
-  Definition get_inf_tree :
+  Unset Implicit Arguments.
+  Unset Contextual Implicit.
+  Definition get_inf_tree' :
     forall (t_fin2 : itree L3 (FinMem.MMEP.MMSP.MemState * (MemPropT.store_id * (local_env * @stack local_env * res_L1)))), itree InfLP.Events.L3 TopLevelBigIntptr.res_L6.
   Proof.
     cofix CIH.
     intros t_fin2.
-    inversion t_fin2.
-    inversion _observe.
+    destruct t_fin2.
+    destruct _observe.
     - (* Ret *)
       refine (ret _).
       destruct r as [ms [sid [[lenv s] [genv res]]]].
@@ -426,7 +428,976 @@ Module InfiniteToFinite.
         inversion H0; subst.
         exact (LLVMEvents.raise H).
       }
+
+      Show Proof.
   Defined.
+
+  Set Printing All.
+  Set Printing Implicit.
+  Set Printing Depth 1000.
+
+
+  Unset Printing All.
+  Unset Printing Implicit.
+  Definition get_inf_tree :
+    forall (t_fin2 : itree L3 (FinMem.MMEP.MMSP.MemState * (MemPropT.store_id * (local_env * @stack local_env * res_L1)))), itree InfLP.Events.L3 TopLevelBigIntptr.res_L6 :=
+cofix CIH (t_fin2 : itree L3 (prod FinMem.MMEP.MMSP.MemState (prod MemPropT.store_id (prod (prod local_env (@stack local_env)) (prod global_env dvalue))))) :
+    itree InfLP.Events.L3
+      (prod InterpreterStackBigIntptr.LLVM.MEM.MMEP.MMSP.MemState (prod MemPropT.store_id (prod (prod InterpreterStackBigIntptr.LLVM.Local.local_env InterpreterStackBigIntptr.LLVM.Stack.lstack) (prod InterpreterStackBigIntptr.LLVM.Global.global_env InterpreterStackBigIntptr.LP.Events.DV.dvalue)))) :=
+  (fun _observe : itreeF L3 (prod FinMem.MMEP.MMSP.MemState (prod MemPropT.store_id (prod (prod local_env (@stack local_env)) (prod global_env dvalue)))) (itree L3 (prod FinMem.MMEP.MMSP.MemState (prod MemPropT.store_id (prod (prod local_env (@stack local_env)) (prod global_env dvalue))))) =>
+   match
+     _observe
+     return
+       (itree InfLP.Events.L3
+          (prod InterpreterStackBigIntptr.LLVM.MEM.MMEP.MMSP.MemState (prod MemPropT.store_id (prod (prod InterpreterStackBigIntptr.LLVM.Local.local_env InterpreterStackBigIntptr.LLVM.Stack.lstack) (prod InterpreterStackBigIntptr.LLVM.Global.global_env InterpreterStackBigIntptr.LP.Events.DV.dvalue)))))
+   with
+   | RetF r =>
+       (fun r0 : prod FinMem.MMEP.MMSP.MemState (prod MemPropT.store_id (prod (prod local_env (@stack local_env)) (prod global_env dvalue))) =>
+        @ret (itree InfLP.Events.L3) (@Monad_itree InfLP.Events.L3)
+          (prod InterpreterStackBigIntptr.LLVM.MEM.MMEP.MMSP.MemState (prod MemPropT.store_id (prod (prod InterpreterStackBigIntptr.LLVM.Local.local_env InterpreterStackBigIntptr.LLVM.Stack.lstack) (prod InterpreterStackBigIntptr.LLVM.Global.global_env InterpreterStackBigIntptr.LP.Events.DV.dvalue))))
+          match
+            r0 return (prod InterpreterStackBigIntptr.LLVM.MEM.MMEP.MMSP.MemState (prod MemPropT.store_id (prod (prod InterpreterStackBigIntptr.LLVM.Local.local_env InterpreterStackBigIntptr.LLVM.Stack.lstack) (prod InterpreterStackBigIntptr.LLVM.Global.global_env InterpreterStackBigIntptr.LP.Events.DV.dvalue))))
+          with
+          | pair a b =>
+              (fun (ms : FinMem.MMEP.MMSP.MemState) (p : prod MemPropT.store_id (prod (prod local_env (@stack local_env)) (prod global_env dvalue))) =>
+               match
+                 p
+                 return
+                   (prod InterpreterStackBigIntptr.LLVM.MEM.MMEP.MMSP.MemState (prod MemPropT.store_id (prod (prod InterpreterStackBigIntptr.LLVM.Local.local_env InterpreterStackBigIntptr.LLVM.Stack.lstack) (prod InterpreterStackBigIntptr.LLVM.Global.global_env InterpreterStackBigIntptr.LP.Events.DV.dvalue))))
+               with
+               | pair a0 b0 =>
+                   (fun (sid : MemPropT.store_id) (p0 : prod (prod local_env (@stack local_env)) (prod global_env dvalue)) =>
+                    match
+                      p0
+                      return
+                        (prod InterpreterStackBigIntptr.LLVM.MEM.MMEP.MMSP.MemState (prod MemPropT.store_id (prod (prod InterpreterStackBigIntptr.LLVM.Local.local_env InterpreterStackBigIntptr.LLVM.Stack.lstack) (prod InterpreterStackBigIntptr.LLVM.Global.global_env InterpreterStackBigIntptr.LP.Events.DV.dvalue))))
+                    with
+                    | pair a1 b1 =>
+                        (fun p1 : prod local_env (@stack local_env) =>
+                         match
+                           p1
+                           return
+                             (forall _ : prod global_env dvalue,
+                              prod InterpreterStackBigIntptr.LLVM.MEM.MMEP.MMSP.MemState
+                                (prod MemPropT.store_id (prod (prod InterpreterStackBigIntptr.LLVM.Local.local_env InterpreterStackBigIntptr.LLVM.Stack.lstack) (prod InterpreterStackBigIntptr.LLVM.Global.global_env InterpreterStackBigIntptr.LP.Events.DV.dvalue))))
+                         with
+                         | pair a2 b2 =>
+                             (fun (lenv : local_env) (s : @stack local_env) (p2 : prod global_env dvalue) =>
+                              match
+                                p2
+                                return
+                                  (prod InterpreterStackBigIntptr.LLVM.MEM.MMEP.MMSP.MemState
+                                     (prod MemPropT.store_id (prod (prod InterpreterStackBigIntptr.LLVM.Local.local_env InterpreterStackBigIntptr.LLVM.Stack.lstack) (prod InterpreterStackBigIntptr.LLVM.Global.global_env InterpreterStackBigIntptr.LP.Events.DV.dvalue))))
+                              with
+                              | pair a3 b3 =>
+                                  (fun (genv : global_env) (res : dvalue) =>
+                                   @pair InterpreterStackBigIntptr.LLVM.MEM.MMEP.MMSP.MemState
+                                     (prod MemPropT.store_id (prod (prod InterpreterStackBigIntptr.LLVM.Local.local_env InterpreterStackBigIntptr.LLVM.Stack.lstack) (prod InterpreterStackBigIntptr.LLVM.Global.global_env InterpreterStackBigIntptr.LP.Events.DV.dvalue))) (lift_MemState ms)
+                                     (@pair MemPropT.store_id (prod (prod InterpreterStackBigIntptr.LLVM.Local.local_env InterpreterStackBigIntptr.LLVM.Stack.lstack) (prod InterpreterStackBigIntptr.LLVM.Global.global_env InterpreterStackBigIntptr.LP.Events.DV.dvalue)) sid
+                                        (@pair (prod InterpreterStackBigIntptr.LLVM.Local.local_env InterpreterStackBigIntptr.LLVM.Stack.lstack) (prod InterpreterStackBigIntptr.LLVM.Global.global_env InterpreterStackBigIntptr.LP.Events.DV.dvalue)
+                                           (@pair InterpreterStackBigIntptr.LLVM.Local.local_env InterpreterStackBigIntptr.LLVM.Stack.lstack (lift_local_env lenv) (lift_stack s))
+                                           (@pair InterpreterStackBigIntptr.LLVM.Global.global_env InterpreterStackBigIntptr.LP.Events.DV.dvalue (lift_global_env genv) (fin_to_inf_dvalue res))))) a3 b3
+                              end) a2 b2
+                         end) a1 b1
+                    end) a0 b0
+               end) a b
+          end) r
+   | TauF t =>
+       (fun t0 : itree L3 (prod FinMem.MMEP.MMSP.MemState (prod MemPropT.store_id (prod (prod local_env (@stack local_env)) (prod global_env dvalue)))) =>
+        @go InfLP.Events.L3
+          (prod InterpreterStackBigIntptr.LLVM.MEM.MMEP.MMSP.MemState (prod MemPropT.store_id (prod (prod InterpreterStackBigIntptr.LLVM.Local.local_env InterpreterStackBigIntptr.LLVM.Stack.lstack) (prod InterpreterStackBigIntptr.LLVM.Global.global_env InterpreterStackBigIntptr.LP.Events.DV.dvalue))))
+          (@TauF InfLP.Events.L3
+             (prod InterpreterStackBigIntptr.LLVM.MEM.MMEP.MMSP.MemState (prod MemPropT.store_id (prod (prod InterpreterStackBigIntptr.LLVM.Local.local_env InterpreterStackBigIntptr.LLVM.Stack.lstack) (prod InterpreterStackBigIntptr.LLVM.Global.global_env InterpreterStackBigIntptr.LP.Events.DV.dvalue))))
+             (itree InfLP.Events.L3
+                (prod InterpreterStackBigIntptr.LLVM.MEM.MMEP.MMSP.MemState (prod MemPropT.store_id (prod (prod InterpreterStackBigIntptr.LLVM.Local.local_env InterpreterStackBigIntptr.LLVM.Stack.lstack) (prod InterpreterStackBigIntptr.LLVM.Global.global_env InterpreterStackBigIntptr.LP.Events.DV.dvalue)))))
+             (CIH t0))) t
+   | @VisF _ _ _ X e k =>
+       (fun (X0 : Type) (e0 : L3 X0) (k0 : forall _ : X0, itree L3 (prod FinMem.MMEP.MMSP.MemState (prod MemPropT.store_id (prod (prod local_env (@stack local_env)) (prod global_env dvalue))))) =>
+        let X1 :
+          itree InfLP.Events.L3
+            (prod InterpreterStackBigIntptr.LLVM.MEM.MMEP.MMSP.MemState (prod MemPropT.store_id (prod (prod InterpreterStackBigIntptr.LLVM.Local.local_env InterpreterStackBigIntptr.LLVM.Stack.lstack) (prod InterpreterStackBigIntptr.LLVM.Global.global_env InterpreterStackBigIntptr.LP.Events.DV.dvalue)))) :=
+          match
+            e0
+            return
+              (itree InfLP.Events.L3
+                 (prod InterpreterStackBigIntptr.LLVM.MEM.MMEP.MMSP.MemState (prod MemPropT.store_id (prod (prod InterpreterStackBigIntptr.LLVM.Local.local_env InterpreterStackBigIntptr.LLVM.Stack.lstack) (prod InterpreterStackBigIntptr.LLVM.Global.global_env InterpreterStackBigIntptr.LP.Events.DV.dvalue)))))
+          with
+          | inl1 x =>
+              (fun H : ExternalCallE X0 =>
+               (fun H0 : ExternalCallE X0 =>
+                let X1 :
+                  forall _ : @eq Type X0 X0,
+                  itree InfLP.Events.L3
+                    (prod InterpreterStackBigIntptr.LLVM.MEM.MMEP.MMSP.MemState (prod MemPropT.store_id (prod (prod InterpreterStackBigIntptr.LLVM.Local.local_env InterpreterStackBigIntptr.LLVM.Stack.lstack) (prod InterpreterStackBigIntptr.LLVM.Global.global_env InterpreterStackBigIntptr.LP.Events.DV.dvalue)))) :=
+                  match
+                    H0 in (ExternalCallE T)
+                    return
+                      (forall _ : @eq Type T X0,
+                       itree InfLP.Events.L3
+                         (prod InterpreterStackBigIntptr.LLVM.MEM.MMEP.MMSP.MemState
+                            (prod MemPropT.store_id (prod (prod InterpreterStackBigIntptr.LLVM.Local.local_env InterpreterStackBigIntptr.LLVM.Stack.lstack) (prod InterpreterStackBigIntptr.LLVM.Global.global_env InterpreterStackBigIntptr.LP.Events.DV.dvalue)))))
+                  with
+                  | ExternalCall t f args =>
+                      (fun (t0 : dtyp) (f0 : uvalue) (args0 : list dvalue) (H1 : @eq Type dvalue X0) =>
+                       (fun H2 : @eq Type dvalue X0 =>
+                        let H3 : @eq Type dvalue X0 := H2 in
+                        @eq_rect Type dvalue
+                          (fun _ : Type =>
+                           forall (_ : dtyp) (_ : uvalue) (_ : list dvalue),
+                           itree InfLP.Events.L3
+                             (prod InterpreterStackBigIntptr.LLVM.MEM.MMEP.MMSP.MemState
+                                (prod MemPropT.store_id (prod (prod InterpreterStackBigIntptr.LLVM.Local.local_env InterpreterStackBigIntptr.LLVM.Stack.lstack) (prod InterpreterStackBigIntptr.LLVM.Global.global_env InterpreterStackBigIntptr.LP.Events.DV.dvalue)))))
+                          (fun (t1 : dtyp) (f1 : uvalue) (args1 : list dvalue) =>
+                           @eq_rect Type dvalue
+                             (fun X1 : Type =>
+                              forall (_ : forall _ : X1, itree L3 (prod FinMem.MMEP.MMSP.MemState (prod MemPropT.store_id (prod (prod local_env (@stack local_env)) (prod global_env dvalue))))) (_ : ExternalCallE X1),
+                              itree InfLP.Events.L3
+                                (prod InterpreterStackBigIntptr.LLVM.MEM.MMEP.MMSP.MemState
+                                   (prod MemPropT.store_id (prod (prod InterpreterStackBigIntptr.LLVM.Local.local_env InterpreterStackBigIntptr.LLVM.Stack.lstack) (prod InterpreterStackBigIntptr.LLVM.Global.global_env InterpreterStackBigIntptr.LP.Events.DV.dvalue)))))
+                             (fun (k1 : forall _ : dvalue, itree L3 (prod FinMem.MMEP.MMSP.MemState (prod MemPropT.store_id (prod (prod local_env (@stack local_env)) (prod global_env dvalue))))) (_ : ExternalCallE dvalue) =>
+                              @go InfLP.Events.L3
+                                (prod InterpreterStackBigIntptr.LLVM.MEM.MMEP.MMSP.MemState
+                                   (prod MemPropT.store_id (prod (prod InterpreterStackBigIntptr.LLVM.Local.local_env InterpreterStackBigIntptr.LLVM.Stack.lstack) (prod InterpreterStackBigIntptr.LLVM.Global.global_env InterpreterStackBigIntptr.LP.Events.DV.dvalue))))
+                                (@VisF InfLP.Events.L3
+                                   (prod InterpreterStackBigIntptr.LLVM.MEM.MMEP.MMSP.MemState
+                                      (prod MemPropT.store_id (prod (prod InterpreterStackBigIntptr.LLVM.Local.local_env InterpreterStackBigIntptr.LLVM.Stack.lstack) (prod InterpreterStackBigIntptr.LLVM.Global.global_env InterpreterStackBigIntptr.LP.Events.DV.dvalue))))
+                                   (itree InfLP.Events.L3
+                                      (prod InterpreterStackBigIntptr.LLVM.MEM.MMEP.MMSP.MemState
+                                         (prod MemPropT.store_id (prod (prod InterpreterStackBigIntptr.LLVM.Local.local_env InterpreterStackBigIntptr.LLVM.Stack.lstack) (prod InterpreterStackBigIntptr.LLVM.Global.global_env InterpreterStackBigIntptr.LP.Events.DV.dvalue))))) E1.DV.dvalue
+                                   (@subevent E1.ExternalCallE InfLP.Events.L3
+                                      (@ReSum_inl (forall _ : Type, Type) IFun sum1 Cat_IFun Inl_sum1 E1.ExternalCallE InfLP.Events.ExternalCallE (sum1 InfLP.Events.PickUvalueE (sum1 OOME (sum1 UBE (sum1 DebugE FailureE)))) (@ReSum_id (forall _ : Type, Type) IFun Id_IFun InfLP.Events.ExternalCallE)) E1.DV.dvalue
+                                      (E1.ExternalCall t1 (fin_to_inf_uvalue f1) (@map LLVMParams64BitIntptr.Events.DV.dvalue LLVMParamsBigIntptr.Events.DV.dvalue fin_to_inf_dvalue args1)))
+                                   (fun x0 : E1.DV.dvalue =>
+                                    CIH
+                                      (let H5 : OOM DVCInfFin.DV2.dvalue := DVCInfFin.dvalue_convert_strict x0 in
+                                       match H5 return (itree L3 (prod FinMem.MMEP.MMSP.MemState (prod MemPropT.store_id (prod (prod local_env (@stack local_env)) (prod global_env dvalue))))) with
+                                       | NoOom a => (fun d : DVCInfFin.DV2.dvalue => k1 d) a
+                                       | Oom s =>
+                                           (fun s0 : string =>
+                                            @raiseOOM L3
+                                              (@ReSum_inr (forall _ : Type, Type) IFun sum1 Cat_IFun Inr_sum1 OOME (sum1 PickUvalueE (sum1 OOME (sum1 UBE (sum1 DebugE FailureE)))) ExternalCallE
+                                                 (@ReSum_inr (forall _ : Type, Type) IFun sum1 Cat_IFun Inr_sum1 OOME (sum1 OOME (sum1 UBE (sum1 DebugE FailureE))) PickUvalueE
+                                                    (@ReSum_inl (forall _ : Type, Type) IFun sum1 Cat_IFun Inl_sum1 OOME OOME (sum1 UBE (sum1 DebugE FailureE)) (@ReSum_id (forall _ : Type, Type) IFun Id_IFun OOME))))
+                                              (prod FinMem.MMEP.MMSP.MemState (prod MemPropT.store_id (prod (prod local_env (@stack local_env)) (prod global_env dvalue)))) s0) s
+                                       end)))) X0 H2 k0 H0) X0 H3) H1 t0 f0 args0) t f args
+                  end in
+                X1 (@eq_refl Type X0)) H) x
+          | inr1 x =>
+              (fun X1 : sum1 PickUvalueE (sum1 OOME (sum1 UBE (sum1 DebugE FailureE))) X0 =>
+               (fun X2 : sum1 PickUvalueE (sum1 OOME (sum1 UBE (sum1 DebugE FailureE))) X0 =>
+                let X3 :
+                  itree InfLP.Events.L3
+                    (prod InterpreterStackBigIntptr.LLVM.MEM.MMEP.MMSP.MemState (prod MemPropT.store_id (prod (prod InterpreterStackBigIntptr.LLVM.Local.local_env InterpreterStackBigIntptr.LLVM.Stack.lstack) (prod InterpreterStackBigIntptr.LLVM.Global.global_env InterpreterStackBigIntptr.LP.Events.DV.dvalue)))) :=
+                  match
+                    X2
+                    return
+                      (itree InfLP.Events.L3
+                         (prod InterpreterStackBigIntptr.LLVM.MEM.MMEP.MMSP.MemState
+                            (prod MemPropT.store_id (prod (prod InterpreterStackBigIntptr.LLVM.Local.local_env InterpreterStackBigIntptr.LLVM.Stack.lstack) (prod InterpreterStackBigIntptr.LLVM.Global.global_env InterpreterStackBigIntptr.LP.Events.DV.dvalue)))))
+                  with
+                  | inl1 x0 =>
+                      (fun X3 : PickUvalueE X0 =>
+                       (fun X4 : PickUvalueE X0 =>
+                        let X5 :
+                          forall _ : @eq Type X0 X0,
+                          itree InfLP.Events.L3
+                            (prod InterpreterStackBigIntptr.LLVM.MEM.MMEP.MMSP.MemState
+                               (prod MemPropT.store_id (prod (prod InterpreterStackBigIntptr.LLVM.Local.local_env InterpreterStackBigIntptr.LLVM.Stack.lstack) (prod InterpreterStackBigIntptr.LLVM.Global.global_env InterpreterStackBigIntptr.LP.Events.DV.dvalue)))) :=
+                          match
+                            X4 in (PickE T)
+                            return
+                              (forall _ : @eq Type T X0,
+                               itree InfLP.Events.L3
+                                 (prod InterpreterStackBigIntptr.LLVM.MEM.MMEP.MMSP.MemState
+                                    (prod MemPropT.store_id (prod (prod InterpreterStackBigIntptr.LLVM.Local.local_env InterpreterStackBigIntptr.LLVM.Stack.lstack) (prod InterpreterStackBigIntptr.LLVM.Global.global_env InterpreterStackBigIntptr.LP.Events.DV.dvalue)))))
+                          with
+                          | pick Pre x1 =>
+                              (fun (Pre0 : Prop) (x2 : uvalue) (H : @eq Type (@sig dvalue (fun _ : dvalue => True)) X0) =>
+                               (fun H0 : @eq Type (@sig dvalue (fun _ : dvalue => True)) X0 =>
+                                let H1 : @eq Type (@sig dvalue (fun _ : dvalue => True)) X0 := H0 in
+                                @eq_rect Type (@sig dvalue (fun _ : dvalue => True))
+                                  (fun _ : Type =>
+                                   forall (_ : Prop) (_ : uvalue),
+                                   itree InfLP.Events.L3
+                                     (prod InterpreterStackBigIntptr.LLVM.MEM.MMEP.MMSP.MemState
+                                        (prod MemPropT.store_id (prod (prod InterpreterStackBigIntptr.LLVM.Local.local_env InterpreterStackBigIntptr.LLVM.Stack.lstack) (prod InterpreterStackBigIntptr.LLVM.Global.global_env InterpreterStackBigIntptr.LP.Events.DV.dvalue)))))
+                                  (fun (Pre1 : Prop) (x3 : uvalue) =>
+                                   @eq_rect Type (@sig dvalue (fun _ : dvalue => True))
+                                     (fun X5 : Type =>
+                                      forall (_ : forall _ : X5, itree L3 (prod FinMem.MMEP.MMSP.MemState (prod MemPropT.store_id (prod (prod local_env (@stack local_env)) (prod global_env dvalue))))) (_ : PickUvalueE X5),
+                                      itree InfLP.Events.L3
+                                        (prod InterpreterStackBigIntptr.LLVM.MEM.MMEP.MMSP.MemState
+                                           (prod MemPropT.store_id (prod (prod InterpreterStackBigIntptr.LLVM.Local.local_env InterpreterStackBigIntptr.LLVM.Stack.lstack) (prod InterpreterStackBigIntptr.LLVM.Global.global_env InterpreterStackBigIntptr.LP.Events.DV.dvalue)))))
+                                     (fun (k1 : forall _ : @sig dvalue (fun _ : dvalue => True), itree L3 (prod FinMem.MMEP.MMSP.MemState (prod MemPropT.store_id (prod (prod local_env (@stack local_env)) (prod global_env dvalue))))) (_ : PickUvalueE (@sig dvalue (fun _ : dvalue => True))) =>
+                                      @go InfLP.Events.L3
+                                        (prod InterpreterStackBigIntptr.LLVM.MEM.MMEP.MMSP.MemState
+                                           (prod MemPropT.store_id (prod (prod InterpreterStackBigIntptr.LLVM.Local.local_env InterpreterStackBigIntptr.LLVM.Stack.lstack) (prod InterpreterStackBigIntptr.LLVM.Global.global_env InterpreterStackBigIntptr.LP.Events.DV.dvalue))))
+                                        (@VisF InfLP.Events.L3
+                                           (prod InterpreterStackBigIntptr.LLVM.MEM.MMEP.MMSP.MemState
+                                              (prod MemPropT.store_id (prod (prod InterpreterStackBigIntptr.LLVM.Local.local_env InterpreterStackBigIntptr.LLVM.Stack.lstack) (prod InterpreterStackBigIntptr.LLVM.Global.global_env InterpreterStackBigIntptr.LP.Events.DV.dvalue))))
+                                           (itree InfLP.Events.L3
+                                              (prod InterpreterStackBigIntptr.LLVM.MEM.MMEP.MMSP.MemState
+                                                 (prod MemPropT.store_id (prod (prod InterpreterStackBigIntptr.LLVM.Local.local_env InterpreterStackBigIntptr.LLVM.Stack.lstack) (prod InterpreterStackBigIntptr.LLVM.Global.global_env InterpreterStackBigIntptr.LP.Events.DV.dvalue)))))
+                                           (@sig InfLP.Events.DV.dvalue (fun _ : InfLP.Events.DV.dvalue => True))
+                                           (@subevent (@E1.PickE LLVMParamsBigIntptr.Events.DV.uvalue InfLP.Events.DV.dvalue (fun (_ : InfLP.Events.DV.uvalue) (_ : InfLP.Events.DV.dvalue) => True)) InfLP.Events.L3
+                                              (@ReSum_inr (forall _ : Type, Type) IFun sum1 Cat_IFun Inr_sum1 (@E1.PickE LLVMParamsBigIntptr.Events.DV.uvalue InfLP.Events.DV.dvalue (fun (_ : InfLP.Events.DV.uvalue) (_ : InfLP.Events.DV.dvalue) => True))
+                                                 (sum1 InfLP.Events.PickUvalueE (sum1 OOME (sum1 UBE (sum1 DebugE FailureE)))) InfLP.Events.ExternalCallE
+                                                 (@ReSum_inl (forall _ : Type, Type) IFun sum1 Cat_IFun Inl_sum1 (@E1.PickE LLVMParamsBigIntptr.Events.DV.uvalue InfLP.Events.DV.dvalue (fun (_ : InfLP.Events.DV.uvalue) (_ : InfLP.Events.DV.dvalue) => True)) InfLP.Events.PickUvalueE
+                                                    (sum1 OOME (sum1 UBE (sum1 DebugE FailureE))) (@ReSum_id (forall _ : Type, Type) IFun Id_IFun InfLP.Events.PickUvalueE))) (@sig InfLP.Events.DV.dvalue (fun _ : InfLP.Events.DV.dvalue => True))
+                                              (@E1.pick LLVMParamsBigIntptr.Events.DV.uvalue InfLP.Events.DV.dvalue (fun (_ : InfLP.Events.DV.uvalue) (_ : InfLP.Events.DV.dvalue) => True) Pre1 (fin_to_inf_uvalue x3)))
+                                           (fun res : @sig InfLP.Events.DV.dvalue (fun _ : InfLP.Events.DV.dvalue => True) =>
+                                            match
+                                              res
+                                              return
+                                                (itree InfLP.Events.L3
+                                                   (prod InterpreterStackBigIntptr.LLVM.MEM.MMEP.MMSP.MemState
+                                                      (prod MemPropT.store_id (prod (prod InterpreterStackBigIntptr.LLVM.Local.local_env InterpreterStackBigIntptr.LLVM.Stack.lstack) (prod InterpreterStackBigIntptr.LLVM.Global.global_env InterpreterStackBigIntptr.LP.Events.DV.dvalue)))))
+                                            with
+                                            | @exist _ _ x4 p =>
+                                                (fun (x5 : InfLP.Events.DV.dvalue) (t : True) =>
+                                                 CIH
+                                                   (let H2 : OOM DVCInfFin.DV2.dvalue := DVCInfFin.dvalue_convert_strict x5 in
+                                                    match H2 return (itree L3 (prod FinMem.MMEP.MMSP.MemState (prod MemPropT.store_id (prod (prod local_env (@stack local_env)) (prod global_env dvalue))))) with
+                                                    | NoOom a => (fun d : DVCInfFin.DV2.dvalue => k1 (@exist dvalue (fun _ : dvalue => True) d t)) a
+                                                    | Oom s =>
+                                                        (fun s0 : string =>
+                                                         @raiseOOM L3
+                                                           (@ReSum_inr (forall _ : Type, Type) IFun sum1 Cat_IFun Inr_sum1 OOME (sum1 PickUvalueE (sum1 OOME (sum1 UBE (sum1 DebugE FailureE)))) ExternalCallE
+                                                              (@ReSum_inr (forall _ : Type, Type) IFun sum1 Cat_IFun Inr_sum1 OOME (sum1 OOME (sum1 UBE (sum1 DebugE FailureE))) PickUvalueE
+                                                                 (@ReSum_inl (forall _ : Type, Type) IFun sum1 Cat_IFun Inl_sum1 OOME OOME (sum1 UBE (sum1 DebugE FailureE)) (@ReSum_id (forall _ : Type, Type) IFun Id_IFun OOME))))
+                                                           (prod FinMem.MMEP.MMSP.MemState (prod MemPropT.store_id (prod (prod local_env (@stack local_env)) (prod global_env dvalue)))) s0) s
+                                                    end)) x4 p
+                                            end))) X0 H0 k0 X4) X0 H1) H Pre0 x2) Pre x1
+                          end in
+                        X5 (@eq_refl Type X0)) X3) x0
+                  | inr1 x0 =>
+                      (fun H : sum1 OOME (sum1 UBE (sum1 DebugE FailureE)) X0 =>
+                       (fun H0 : sum1 OOME (sum1 UBE (sum1 DebugE FailureE)) X0 =>
+                        let X3 :
+                          itree InfLP.Events.L3
+                            (prod InterpreterStackBigIntptr.LLVM.MEM.MMEP.MMSP.MemState
+                               (prod MemPropT.store_id (prod (prod InterpreterStackBigIntptr.LLVM.Local.local_env InterpreterStackBigIntptr.LLVM.Stack.lstack) (prod InterpreterStackBigIntptr.LLVM.Global.global_env InterpreterStackBigIntptr.LP.Events.DV.dvalue)))) :=
+                          match
+                            H0
+                            return
+                              (itree InfLP.Events.L3
+                                 (prod InterpreterStackBigIntptr.LLVM.MEM.MMEP.MMSP.MemState
+                                    (prod MemPropT.store_id (prod (prod InterpreterStackBigIntptr.LLVM.Local.local_env InterpreterStackBigIntptr.LLVM.Stack.lstack) (prod InterpreterStackBigIntptr.LLVM.Global.global_env InterpreterStackBigIntptr.LP.Events.DV.dvalue)))))
+                          with
+                          | inl1 x1 =>
+                              (fun H1 : OOME X0 =>
+                               (fun H2 : OOME X0 =>
+                                let X3 :
+                                  forall _ : @eq Type X0 X0,
+                                  itree InfLP.Events.L3
+                                    (prod InterpreterStackBigIntptr.LLVM.MEM.MMEP.MMSP.MemState
+                                       (prod MemPropT.store_id (prod (prod InterpreterStackBigIntptr.LLVM.Local.local_env InterpreterStackBigIntptr.LLVM.Stack.lstack) (prod InterpreterStackBigIntptr.LLVM.Global.global_env InterpreterStackBigIntptr.LP.Events.DV.dvalue)))) :=
+                                  match
+                                    H2 in (OOME T)
+                                    return
+                                      (forall _ : @eq Type T X0,
+                                       itree InfLP.Events.L3
+                                         (prod InterpreterStackBigIntptr.LLVM.MEM.MMEP.MMSP.MemState
+                                            (prod MemPropT.store_id (prod (prod InterpreterStackBigIntptr.LLVM.Local.local_env InterpreterStackBigIntptr.LLVM.Stack.lstack) (prod InterpreterStackBigIntptr.LLVM.Global.global_env InterpreterStackBigIntptr.LP.Events.DV.dvalue)))))
+                                  with
+                                  | ThrowOOM x2 =>
+                                      (fun (H3 : string) (H4 : @eq Type Empty_set X0) =>
+                                       (fun H5 : @eq Type Empty_set X0 =>
+                                        let H6 : @eq Type Empty_set X0 := H5 in
+                                        @eq_rect Type Empty_set
+                                          (fun _ : Type =>
+                                           forall _ : string,
+                                           itree InfLP.Events.L3
+                                             (prod InterpreterStackBigIntptr.LLVM.MEM.MMEP.MMSP.MemState
+                                                (prod MemPropT.store_id (prod (prod InterpreterStackBigIntptr.LLVM.Local.local_env InterpreterStackBigIntptr.LLVM.Stack.lstack) (prod InterpreterStackBigIntptr.LLVM.Global.global_env InterpreterStackBigIntptr.LP.Events.DV.dvalue)))))
+                                          (fun H7 : string =>
+                                           @eq_rect Type Empty_set
+                                             (fun X3 : Type =>
+                                              forall (_ : forall _ : X3, itree L3 (prod FinMem.MMEP.MMSP.MemState (prod MemPropT.store_id (prod (prod local_env (@stack local_env)) (prod global_env dvalue))))) (_ : OOME X3),
+                                              itree InfLP.Events.L3
+                                                (prod InterpreterStackBigIntptr.LLVM.MEM.MMEP.MMSP.MemState
+                                                   (prod MemPropT.store_id (prod (prod InterpreterStackBigIntptr.LLVM.Local.local_env InterpreterStackBigIntptr.LLVM.Stack.lstack) (prod InterpreterStackBigIntptr.LLVM.Global.global_env InterpreterStackBigIntptr.LP.Events.DV.dvalue)))))
+                                             (fun (_ : forall _ : Empty_set, itree L3 (prod FinMem.MMEP.MMSP.MemState (prod MemPropT.store_id (prod (prod local_env (@stack local_env)) (prod global_env dvalue))))) (_ : OOME Empty_set) =>
+                                              @raiseOOM InfLP.Events.L3
+                                                (@ReSum_inr (forall _ : Type, Type) IFun sum1 Cat_IFun Inr_sum1 OOME (sum1 InfLP.Events.PickUvalueE (sum1 OOME (sum1 UBE (sum1 DebugE FailureE)))) InfLP.Events.ExternalCallE
+                                                   (@ReSum_inr (forall _ : Type, Type) IFun sum1 Cat_IFun Inr_sum1 OOME (sum1 OOME (sum1 UBE (sum1 DebugE FailureE))) InfLP.Events.PickUvalueE
+                                                      (@ReSum_inl (forall _ : Type, Type) IFun sum1 Cat_IFun Inl_sum1 OOME OOME (sum1 UBE (sum1 DebugE FailureE)) (@ReSum_id (forall _ : Type, Type) IFun Id_IFun OOME))))
+                                                (prod InterpreterStackBigIntptr.LLVM.MEM.MMEP.MMSP.MemState
+                                                   (prod MemPropT.store_id (prod (prod InterpreterStackBigIntptr.LLVM.Local.local_env InterpreterStackBigIntptr.LLVM.Stack.lstack) (prod InterpreterStackBigIntptr.LLVM.Global.global_env InterpreterStackBigIntptr.LP.Events.DV.dvalue)))) H7) X0 H5 k0 H2) X0 H6) H4 H3)
+                                        x2
+                                  end in
+                                X3 (@eq_refl Type X0)) H1) x1
+                          | inr1 x1 =>
+                              (fun H1 : sum1 UBE (sum1 DebugE FailureE) X0 =>
+                               (fun H2 : sum1 UBE (sum1 DebugE FailureE) X0 =>
+                                let X3 :
+                                  itree InfLP.Events.L3
+                                    (prod InterpreterStackBigIntptr.LLVM.MEM.MMEP.MMSP.MemState
+                                       (prod MemPropT.store_id (prod (prod InterpreterStackBigIntptr.LLVM.Local.local_env InterpreterStackBigIntptr.LLVM.Stack.lstack) (prod InterpreterStackBigIntptr.LLVM.Global.global_env InterpreterStackBigIntptr.LP.Events.DV.dvalue)))) :=
+                                  match
+                                    H2
+                                    return
+                                      (itree InfLP.Events.L3
+                                         (prod InterpreterStackBigIntptr.LLVM.MEM.MMEP.MMSP.MemState
+                                            (prod MemPropT.store_id (prod (prod InterpreterStackBigIntptr.LLVM.Local.local_env InterpreterStackBigIntptr.LLVM.Stack.lstack) (prod InterpreterStackBigIntptr.LLVM.Global.global_env InterpreterStackBigIntptr.LP.Events.DV.dvalue)))))
+                                  with
+                                  | inl1 x2 =>
+                                      (fun H3 : UBE X0 =>
+                                       (fun H4 : UBE X0 =>
+                                        let X3 :
+                                          forall _ : @eq Type X0 X0,
+                                          itree InfLP.Events.L3
+                                            (prod InterpreterStackBigIntptr.LLVM.MEM.MMEP.MMSP.MemState
+                                               (prod MemPropT.store_id (prod (prod InterpreterStackBigIntptr.LLVM.Local.local_env InterpreterStackBigIntptr.LLVM.Stack.lstack) (prod InterpreterStackBigIntptr.LLVM.Global.global_env InterpreterStackBigIntptr.LP.Events.DV.dvalue)))) :=
+                                          match
+                                            H4 in (UBE T)
+                                            return
+                                              (forall _ : @eq Type T X0,
+                                               itree InfLP.Events.L3
+                                                 (prod InterpreterStackBigIntptr.LLVM.MEM.MMEP.MMSP.MemState
+                                                    (prod MemPropT.store_id (prod (prod InterpreterStackBigIntptr.LLVM.Local.local_env InterpreterStackBigIntptr.LLVM.Stack.lstack) (prod InterpreterStackBigIntptr.LLVM.Global.global_env InterpreterStackBigIntptr.LP.Events.DV.dvalue)))))
+                                          with
+                                          | ThrowUB x3 =>
+                                              (fun (H5 : string) (H6 : @eq Type Empty_set X0) =>
+                                               (fun H7 : @eq Type Empty_set X0 =>
+                                                let H8 : @eq Type Empty_set X0 := H7 in
+                                                @eq_rect Type Empty_set
+                                                  (fun _ : Type =>
+                                                   forall _ : string,
+                                                   itree InfLP.Events.L3
+                                                     (prod InterpreterStackBigIntptr.LLVM.MEM.MMEP.MMSP.MemState
+                                                        (prod MemPropT.store_id (prod (prod InterpreterStackBigIntptr.LLVM.Local.local_env InterpreterStackBigIntptr.LLVM.Stack.lstack) (prod InterpreterStackBigIntptr.LLVM.Global.global_env InterpreterStackBigIntptr.LP.Events.DV.dvalue)))))
+                                                  (fun H9 : string =>
+                                                   @eq_rect Type Empty_set
+                                                     (fun X3 : Type =>
+                                                      forall (_ : forall _ : X3, itree L3 (prod FinMem.MMEP.MMSP.MemState (prod MemPropT.store_id (prod (prod local_env (@stack local_env)) (prod global_env dvalue))))) (_ : UBE X3),
+                                                      itree InfLP.Events.L3
+                                                        (prod InterpreterStackBigIntptr.LLVM.MEM.MMEP.MMSP.MemState
+                                                           (prod MemPropT.store_id (prod (prod InterpreterStackBigIntptr.LLVM.Local.local_env InterpreterStackBigIntptr.LLVM.Stack.lstack) (prod InterpreterStackBigIntptr.LLVM.Global.global_env InterpreterStackBigIntptr.LP.Events.DV.dvalue)))))
+                                                     (fun (_ : forall _ : Empty_set, itree L3 (prod FinMem.MMEP.MMSP.MemState (prod MemPropT.store_id (prod (prod local_env (@stack local_env)) (prod global_env dvalue))))) (_ : UBE Empty_set) =>
+                                                      @raiseUB InfLP.Events.L3
+                                                        (@ReSum_inr (forall _ : Type, Type) IFun sum1 Cat_IFun Inr_sum1 UBE (sum1 InfLP.Events.PickUvalueE (sum1 OOME (sum1 UBE (sum1 DebugE FailureE)))) InfLP.Events.ExternalCallE
+                                                           (@ReSum_inr (forall _ : Type, Type) IFun sum1 Cat_IFun Inr_sum1 UBE (sum1 OOME (sum1 UBE (sum1 DebugE FailureE))) InfLP.Events.PickUvalueE
+                                                              (@ReSum_inr (forall _ : Type, Type) IFun sum1 Cat_IFun Inr_sum1 UBE (sum1 UBE (sum1 DebugE FailureE)) OOME
+                                                                 (@ReSum_inl (forall _ : Type, Type) IFun sum1 Cat_IFun Inl_sum1 UBE UBE (sum1 DebugE FailureE) (@ReSum_id (forall _ : Type, Type) IFun Id_IFun UBE)))))
+                                                        (prod InterpreterStackBigIntptr.LLVM.MEM.MMEP.MMSP.MemState
+                                                           (prod MemPropT.store_id (prod (prod InterpreterStackBigIntptr.LLVM.Local.local_env InterpreterStackBigIntptr.LLVM.Stack.lstack) (prod InterpreterStackBigIntptr.LLVM.Global.global_env InterpreterStackBigIntptr.LP.Events.DV.dvalue)))) H9) X0 H7 k0 H4) X0 H8)
+                                                 H6 H5) x3
+                                          end in
+                                        X3 (@eq_refl Type X0)) H3) x2
+                                  | inr1 x2 =>
+                                      (fun H3 : sum1 DebugE FailureE X0 =>
+                                       (fun H4 : sum1 DebugE FailureE X0 =>
+                                        let X3 :
+                                          itree InfLP.Events.L3
+                                            (prod InterpreterStackBigIntptr.LLVM.MEM.MMEP.MMSP.MemState
+                                               (prod MemPropT.store_id (prod (prod InterpreterStackBigIntptr.LLVM.Local.local_env InterpreterStackBigIntptr.LLVM.Stack.lstack) (prod InterpreterStackBigIntptr.LLVM.Global.global_env InterpreterStackBigIntptr.LP.Events.DV.dvalue)))) :=
+                                          match
+                                            H4
+                                            return
+                                              (itree InfLP.Events.L3
+                                                 (prod InterpreterStackBigIntptr.LLVM.MEM.MMEP.MMSP.MemState
+                                                    (prod MemPropT.store_id (prod (prod InterpreterStackBigIntptr.LLVM.Local.local_env InterpreterStackBigIntptr.LLVM.Stack.lstack) (prod InterpreterStackBigIntptr.LLVM.Global.global_env InterpreterStackBigIntptr.LP.Events.DV.dvalue)))))
+                                          with
+                                          | inl1 x3 =>
+                                              (fun H5 : DebugE X0 =>
+                                               (fun H6 : DebugE X0 =>
+                                                let X3 :
+                                                  forall _ : @eq Type X0 X0,
+                                                  itree InfLP.Events.L3
+                                                    (prod InterpreterStackBigIntptr.LLVM.MEM.MMEP.MMSP.MemState
+                                                       (prod MemPropT.store_id (prod (prod InterpreterStackBigIntptr.LLVM.Local.local_env InterpreterStackBigIntptr.LLVM.Stack.lstack) (prod InterpreterStackBigIntptr.LLVM.Global.global_env InterpreterStackBigIntptr.LP.Events.DV.dvalue)))) :=
+                                                  match
+                                                    H6 in (DebugE T)
+                                                    return
+                                                      (forall _ : @eq Type T X0,
+                                                       itree InfLP.Events.L3
+                                                         (prod InterpreterStackBigIntptr.LLVM.MEM.MMEP.MMSP.MemState
+                                                            (prod MemPropT.store_id (prod (prod InterpreterStackBigIntptr.LLVM.Local.local_env InterpreterStackBigIntptr.LLVM.Stack.lstack) (prod InterpreterStackBigIntptr.LLVM.Global.global_env InterpreterStackBigIntptr.LP.Events.DV.dvalue)))))
+                                                  with
+                                                  | Debug x4 =>
+                                                      (fun (H7 : string) (H8 : @eq Type unit X0) =>
+                                                       (fun H9 : @eq Type unit X0 =>
+                                                        let H10 : @eq Type unit X0 := H9 in
+                                                        @eq_rect Type unit
+                                                          (fun _ : Type =>
+                                                           forall _ : string,
+                                                           itree InfLP.Events.L3
+                                                             (prod InterpreterStackBigIntptr.LLVM.MEM.MMEP.MMSP.MemState
+                                                                (prod MemPropT.store_id (prod (prod InterpreterStackBigIntptr.LLVM.Local.local_env InterpreterStackBigIntptr.LLVM.Stack.lstack) (prod InterpreterStackBigIntptr.LLVM.Global.global_env InterpreterStackBigIntptr.LP.Events.DV.dvalue)))))
+                                                          (fun H11 : string =>
+                                                           @eq_rect Type unit
+                                                             (fun X3 : Type =>
+                                                              forall (_ : forall _ : X3, itree L3 (prod FinMem.MMEP.MMSP.MemState (prod MemPropT.store_id (prod (prod local_env (@stack local_env)) (prod global_env dvalue))))) (_ : DebugE X3),
+                                                              itree InfLP.Events.L3
+                                                                (prod InterpreterStackBigIntptr.LLVM.MEM.MMEP.MMSP.MemState
+                                                                   (prod MemPropT.store_id (prod (prod InterpreterStackBigIntptr.LLVM.Local.local_env InterpreterStackBigIntptr.LLVM.Stack.lstack) (prod InterpreterStackBigIntptr.LLVM.Global.global_env InterpreterStackBigIntptr.LP.Events.DV.dvalue)))))
+                                                             (fun (k1 : forall _ : unit, itree L3 (prod FinMem.MMEP.MMSP.MemState (prod MemPropT.store_id (prod (prod local_env (@stack local_env)) (prod global_env dvalue))))) (_ : DebugE unit) =>
+                                                              @go InfLP.Events.L3
+                                                                (prod InterpreterStackBigIntptr.LLVM.MEM.MMEP.MMSP.MemState
+                                                                   (prod MemPropT.store_id (prod (prod InterpreterStackBigIntptr.LLVM.Local.local_env InterpreterStackBigIntptr.LLVM.Stack.lstack) (prod InterpreterStackBigIntptr.LLVM.Global.global_env InterpreterStackBigIntptr.LP.Events.DV.dvalue))))
+                                                                (@VisF InfLP.Events.L3
+                                                                   (prod InterpreterStackBigIntptr.LLVM.MEM.MMEP.MMSP.MemState
+                                                                      (prod MemPropT.store_id (prod (prod InterpreterStackBigIntptr.LLVM.Local.local_env InterpreterStackBigIntptr.LLVM.Stack.lstack) (prod InterpreterStackBigIntptr.LLVM.Global.global_env InterpreterStackBigIntptr.LP.Events.DV.dvalue))))
+                                                                   (itree InfLP.Events.L3
+                                                                      (prod InterpreterStackBigIntptr.LLVM.MEM.MMEP.MMSP.MemState
+                                                                         (prod MemPropT.store_id (prod (prod InterpreterStackBigIntptr.LLVM.Local.local_env InterpreterStackBigIntptr.LLVM.Stack.lstack) (prod InterpreterStackBigIntptr.LLVM.Global.global_env InterpreterStackBigIntptr.LP.Events.DV.dvalue))))) unit
+                                                                   (@subevent DebugE InfLP.Events.L3
+                                                                      (@ReSum_inr (forall _ : Type, Type) IFun sum1 Cat_IFun Inr_sum1 DebugE (sum1 InfLP.Events.PickUvalueE (sum1 OOME (sum1 UBE (sum1 DebugE FailureE)))) InfLP.Events.ExternalCallE
+                                                                         (@ReSum_inr (forall _ : Type, Type) IFun sum1 Cat_IFun Inr_sum1 DebugE (sum1 OOME (sum1 UBE (sum1 DebugE FailureE))) InfLP.Events.PickUvalueE
+                                                                            (@ReSum_inr (forall _ : Type, Type) IFun sum1 Cat_IFun Inr_sum1 DebugE (sum1 UBE (sum1 DebugE FailureE)) OOME
+                                                                               (@ReSum_inr (forall _ : Type, Type) IFun sum1 Cat_IFun Inr_sum1 DebugE (sum1 DebugE FailureE) UBE
+                                                                                  (@ReSum_inl (forall _ : Type, Type) IFun sum1 Cat_IFun Inl_sum1 DebugE DebugE FailureE (@ReSum_id (forall _ : Type, Type) IFun Id_IFun DebugE)))))) unit (Debug H11)) (fun H13 : unit => CIH (k1 H13)))) X0 H9 k0 H6) X0 H10) H8 H7) x4
+                                                  end in
+                                                X3 (@eq_refl Type X0)) H5) x3
+                                          | inr1 x3 =>
+                                              (fun H5 : FailureE X0 =>
+                                               (fun H6 : FailureE X0 =>
+                                                let X3 :
+                                                  forall _ : @eq Type X0 X0,
+                                                  itree InfLP.Events.L3
+                                                    (prod InterpreterStackBigIntptr.LLVM.MEM.MMEP.MMSP.MemState
+                                                       (prod MemPropT.store_id (prod (prod InterpreterStackBigIntptr.LLVM.Local.local_env InterpreterStackBigIntptr.LLVM.Stack.lstack) (prod InterpreterStackBigIntptr.LLVM.Global.global_env InterpreterStackBigIntptr.LP.Events.DV.dvalue)))) :=
+                                                  match
+                                                    H6 in (FailureE T)
+                                                    return
+                                                      (forall _ : @eq Type T X0,
+                                                       itree InfLP.Events.L3
+                                                         (prod InterpreterStackBigIntptr.LLVM.MEM.MMEP.MMSP.MemState
+                                                            (prod MemPropT.store_id (prod (prod InterpreterStackBigIntptr.LLVM.Local.local_env InterpreterStackBigIntptr.LLVM.Stack.lstack) (prod InterpreterStackBigIntptr.LLVM.Global.global_env InterpreterStackBigIntptr.LP.Events.DV.dvalue)))))
+                                                  with
+                                                  | Throw x4 =>
+                                                      (fun (H7 : string) (H8 : @eq Type Empty_set X0) =>
+                                                       (fun H9 : @eq Type Empty_set X0 =>
+                                                        let H10 : @eq Type Empty_set X0 := H9 in
+                                                        @eq_rect Type Empty_set
+                                                          (fun _ : Type =>
+                                                           forall _ : string,
+                                                           itree InfLP.Events.L3
+                                                             (prod InterpreterStackBigIntptr.LLVM.MEM.MMEP.MMSP.MemState
+                                                                (prod MemPropT.store_id (prod (prod InterpreterStackBigIntptr.LLVM.Local.local_env InterpreterStackBigIntptr.LLVM.Stack.lstack) (prod InterpreterStackBigIntptr.LLVM.Global.global_env InterpreterStackBigIntptr.LP.Events.DV.dvalue)))))
+                                                          (fun H11 : string =>
+                                                           @eq_rect Type Empty_set
+                                                             (fun X3 : Type =>
+                                                              forall (_ : forall _ : X3, itree L3 (prod FinMem.MMEP.MMSP.MemState (prod MemPropT.store_id (prod (prod local_env (@stack local_env)) (prod global_env dvalue))))) (_ : FailureE X3),
+                                                              itree InfLP.Events.L3
+                                                                (prod InterpreterStackBigIntptr.LLVM.MEM.MMEP.MMSP.MemState
+                                                                   (prod MemPropT.store_id (prod (prod InterpreterStackBigIntptr.LLVM.Local.local_env InterpreterStackBigIntptr.LLVM.Stack.lstack) (prod InterpreterStackBigIntptr.LLVM.Global.global_env InterpreterStackBigIntptr.LP.Events.DV.dvalue)))))
+                                                             (fun (_ : forall _ : Empty_set, itree L3 (prod FinMem.MMEP.MMSP.MemState (prod MemPropT.store_id (prod (prod local_env (@stack local_env)) (prod global_env dvalue))))) (_ : FailureE Empty_set) =>
+                                                              @LLVMEvents.raise InfLP.Events.L3
+                                                                (prod InterpreterStackBigIntptr.LLVM.MEM.MMEP.MMSP.MemState
+                                                                   (prod MemPropT.store_id (prod (prod InterpreterStackBigIntptr.LLVM.Local.local_env InterpreterStackBigIntptr.LLVM.Stack.lstack) (prod InterpreterStackBigIntptr.LLVM.Global.global_env InterpreterStackBigIntptr.LP.Events.DV.dvalue))))
+                                                                (@ReSum_inr (forall _ : Type, Type) IFun sum1 Cat_IFun Inr_sum1 FailureE (sum1 InfLP.Events.PickUvalueE (sum1 OOME (sum1 UBE (sum1 DebugE FailureE)))) InfLP.Events.ExternalCallE
+                                                                   (@ReSum_inr (forall _ : Type, Type) IFun sum1 Cat_IFun Inr_sum1 FailureE (sum1 OOME (sum1 UBE (sum1 DebugE FailureE))) InfLP.Events.PickUvalueE
+                                                                      (@ReSum_inr (forall _ : Type, Type) IFun sum1 Cat_IFun Inr_sum1 FailureE (sum1 UBE (sum1 DebugE FailureE)) OOME
+                                                                         (@ReSum_inr (forall _ : Type, Type) IFun sum1 Cat_IFun Inr_sum1 FailureE (sum1 DebugE FailureE) UBE
+                                                                            (@ReSum_inr (forall _ : Type, Type) IFun sum1 Cat_IFun Inr_sum1 FailureE FailureE DebugE (@ReSum_id (forall _ : Type, Type) IFun Id_IFun FailureE)))))) H11) X0 H9 k0 H6) X0 H10) H8 H7) x4
+                                                  end in
+                                                X3 (@eq_refl Type X0)) H5) x3
+                                          end in
+                                        X3) H3) x2
+                                  end in
+                                X3) H1) x1
+                          end in
+                        X3) H) x0
+                  end in
+                X3) X1) x
+          end in
+        X1) X e k
+   end) (@_observe _ _ t_fin2).
+
+  Definition _get_inf_tree (t_fin2 : itree' L3 (FinMem.MMEP.MMSP.MemState * (MemPropT.store_id * (local_env * @stack local_env * res_L1)))) : itree InfLP.Events.L3 TopLevelBigIntptr.res_L6 :=
+    match t_fin2 with
+    | RetF r =>
+        (fun r0 : prod FinMem.MMEP.MMSP.MemState (prod MemPropT.store_id (prod (prod local_env (@stack local_env)) (prod global_env dvalue))) =>
+           @ret (itree InfLP.Events.L3) (@Monad_itree InfLP.Events.L3)
+             (prod InterpreterStackBigIntptr.LLVM.MEM.MMEP.MMSP.MemState (prod MemPropT.store_id (prod (prod InterpreterStackBigIntptr.LLVM.Local.local_env InterpreterStackBigIntptr.LLVM.Stack.lstack) (prod InterpreterStackBigIntptr.LLVM.Global.global_env InterpreterStackBigIntptr.LP.Events.DV.dvalue))))
+             match
+               r0 return (prod InterpreterStackBigIntptr.LLVM.MEM.MMEP.MMSP.MemState (prod MemPropT.store_id (prod (prod InterpreterStackBigIntptr.LLVM.Local.local_env InterpreterStackBigIntptr.LLVM.Stack.lstack) (prod InterpreterStackBigIntptr.LLVM.Global.global_env InterpreterStackBigIntptr.LP.Events.DV.dvalue))))
+             with
+             | pair a b =>
+                 (fun (ms : FinMem.MMEP.MMSP.MemState) (p : prod MemPropT.store_id (prod (prod local_env (@stack local_env)) (prod global_env dvalue))) =>
+                    match
+                      p
+                      return
+                      (prod InterpreterStackBigIntptr.LLVM.MEM.MMEP.MMSP.MemState (prod MemPropT.store_id (prod (prod InterpreterStackBigIntptr.LLVM.Local.local_env InterpreterStackBigIntptr.LLVM.Stack.lstack) (prod InterpreterStackBigIntptr.LLVM.Global.global_env InterpreterStackBigIntptr.LP.Events.DV.dvalue))))
+                    with
+                    | pair a0 b0 =>
+                        (fun (sid : MemPropT.store_id) (p0 : prod (prod local_env (@stack local_env)) (prod global_env dvalue)) =>
+                           match
+                             p0
+                             return
+                             (prod InterpreterStackBigIntptr.LLVM.MEM.MMEP.MMSP.MemState (prod MemPropT.store_id (prod (prod InterpreterStackBigIntptr.LLVM.Local.local_env InterpreterStackBigIntptr.LLVM.Stack.lstack) (prod InterpreterStackBigIntptr.LLVM.Global.global_env InterpreterStackBigIntptr.LP.Events.DV.dvalue))))
+                           with
+                           | pair a1 b1 =>
+                               (fun p1 : prod local_env (@stack local_env) =>
+                                  match
+                                    p1
+                                    return
+                                    (forall _ : prod global_env dvalue,
+                                        prod InterpreterStackBigIntptr.LLVM.MEM.MMEP.MMSP.MemState
+                                          (prod MemPropT.store_id (prod (prod InterpreterStackBigIntptr.LLVM.Local.local_env InterpreterStackBigIntptr.LLVM.Stack.lstack) (prod InterpreterStackBigIntptr.LLVM.Global.global_env InterpreterStackBigIntptr.LP.Events.DV.dvalue))))
+                                  with
+                                  | pair a2 b2 =>
+                                      (fun (lenv : local_env) (s : @stack local_env) (p2 : prod global_env dvalue) =>
+                                         match
+                                           p2
+                                           return
+                                           (prod InterpreterStackBigIntptr.LLVM.MEM.MMEP.MMSP.MemState
+                                              (prod MemPropT.store_id (prod (prod InterpreterStackBigIntptr.LLVM.Local.local_env InterpreterStackBigIntptr.LLVM.Stack.lstack) (prod InterpreterStackBigIntptr.LLVM.Global.global_env InterpreterStackBigIntptr.LP.Events.DV.dvalue))))
+                                         with
+                                         | pair a3 b3 =>
+                                             (fun (genv : global_env) (res : dvalue) =>
+                                                @pair InterpreterStackBigIntptr.LLVM.MEM.MMEP.MMSP.MemState
+                                                  (prod MemPropT.store_id (prod (prod InterpreterStackBigIntptr.LLVM.Local.local_env InterpreterStackBigIntptr.LLVM.Stack.lstack) (prod InterpreterStackBigIntptr.LLVM.Global.global_env InterpreterStackBigIntptr.LP.Events.DV.dvalue))) (lift_MemState ms)
+                                                  (@pair MemPropT.store_id (prod (prod InterpreterStackBigIntptr.LLVM.Local.local_env InterpreterStackBigIntptr.LLVM.Stack.lstack) (prod InterpreterStackBigIntptr.LLVM.Global.global_env InterpreterStackBigIntptr.LP.Events.DV.dvalue)) sid
+                                                     (@pair (prod InterpreterStackBigIntptr.LLVM.Local.local_env InterpreterStackBigIntptr.LLVM.Stack.lstack) (prod InterpreterStackBigIntptr.LLVM.Global.global_env InterpreterStackBigIntptr.LP.Events.DV.dvalue)
+                                                        (@pair InterpreterStackBigIntptr.LLVM.Local.local_env InterpreterStackBigIntptr.LLVM.Stack.lstack (lift_local_env lenv) (lift_stack s))
+                                                        (@pair InterpreterStackBigIntptr.LLVM.Global.global_env InterpreterStackBigIntptr.LP.Events.DV.dvalue (lift_global_env genv) (fin_to_inf_dvalue res))))) a3 b3
+                                         end) a2 b2
+                                  end) a1 b1
+                           end) a0 b0
+                    end) a b
+             end) r
+    | TauF t =>
+        (fun t0 : itree L3 (prod FinMem.MMEP.MMSP.MemState (prod MemPropT.store_id (prod (prod local_env (@stack local_env)) (prod global_env dvalue)))) =>
+           @go InfLP.Events.L3
+             (prod InterpreterStackBigIntptr.LLVM.MEM.MMEP.MMSP.MemState (prod MemPropT.store_id (prod (prod InterpreterStackBigIntptr.LLVM.Local.local_env InterpreterStackBigIntptr.LLVM.Stack.lstack) (prod InterpreterStackBigIntptr.LLVM.Global.global_env InterpreterStackBigIntptr.LP.Events.DV.dvalue))))
+             (@TauF InfLP.Events.L3
+                (prod InterpreterStackBigIntptr.LLVM.MEM.MMEP.MMSP.MemState (prod MemPropT.store_id (prod (prod InterpreterStackBigIntptr.LLVM.Local.local_env InterpreterStackBigIntptr.LLVM.Stack.lstack) (prod InterpreterStackBigIntptr.LLVM.Global.global_env InterpreterStackBigIntptr.LP.Events.DV.dvalue))))
+                (itree InfLP.Events.L3
+                   (prod InterpreterStackBigIntptr.LLVM.MEM.MMEP.MMSP.MemState (prod MemPropT.store_id (prod (prod InterpreterStackBigIntptr.LLVM.Local.local_env InterpreterStackBigIntptr.LLVM.Stack.lstack) (prod InterpreterStackBigIntptr.LLVM.Global.global_env InterpreterStackBigIntptr.LP.Events.DV.dvalue)))))
+                (get_inf_tree t0))) t
+    | VisF X e k =>
+       (fun (X0 : Type) (e0 : L3 X0) (k0 : forall _ : X0, itree L3 (prod FinMem.MMEP.MMSP.MemState (prod MemPropT.store_id (prod (prod local_env (@stack local_env)) (prod global_env dvalue))))) =>
+        let X1 :
+          itree InfLP.Events.L3
+            (prod InterpreterStackBigIntptr.LLVM.MEM.MMEP.MMSP.MemState (prod MemPropT.store_id (prod (prod InterpreterStackBigIntptr.LLVM.Local.local_env InterpreterStackBigIntptr.LLVM.Stack.lstack) (prod InterpreterStackBigIntptr.LLVM.Global.global_env InterpreterStackBigIntptr.LP.Events.DV.dvalue)))) :=
+          match
+            e0
+            return
+              (itree InfLP.Events.L3
+                 (prod InterpreterStackBigIntptr.LLVM.MEM.MMEP.MMSP.MemState (prod MemPropT.store_id (prod (prod InterpreterStackBigIntptr.LLVM.Local.local_env InterpreterStackBigIntptr.LLVM.Stack.lstack) (prod InterpreterStackBigIntptr.LLVM.Global.global_env InterpreterStackBigIntptr.LP.Events.DV.dvalue)))))
+          with
+          | inl1 x =>
+              (fun H : ExternalCallE X0 =>
+               (fun H0 : ExternalCallE X0 =>
+                let X1 :
+                  forall _ : @eq Type X0 X0,
+                  itree InfLP.Events.L3
+                    (prod InterpreterStackBigIntptr.LLVM.MEM.MMEP.MMSP.MemState (prod MemPropT.store_id (prod (prod InterpreterStackBigIntptr.LLVM.Local.local_env InterpreterStackBigIntptr.LLVM.Stack.lstack) (prod InterpreterStackBigIntptr.LLVM.Global.global_env InterpreterStackBigIntptr.LP.Events.DV.dvalue)))) :=
+                  match
+                    H0 in (ExternalCallE T)
+                    return
+                      (forall _ : @eq Type T X0,
+                       itree InfLP.Events.L3
+                         (prod InterpreterStackBigIntptr.LLVM.MEM.MMEP.MMSP.MemState
+                            (prod MemPropT.store_id (prod (prod InterpreterStackBigIntptr.LLVM.Local.local_env InterpreterStackBigIntptr.LLVM.Stack.lstack) (prod InterpreterStackBigIntptr.LLVM.Global.global_env InterpreterStackBigIntptr.LP.Events.DV.dvalue)))))
+                  with
+                  | ExternalCall t f args =>
+                      (fun (t0 : dtyp) (f0 : uvalue) (args0 : list dvalue) (H1 : @eq Type dvalue X0) =>
+                       (fun H2 : @eq Type dvalue X0 =>
+                        let H3 : @eq Type dvalue X0 := H2 in
+                        @eq_rect Type dvalue
+                          (fun _ : Type =>
+                           forall (_ : dtyp) (_ : uvalue) (_ : list dvalue),
+                           itree InfLP.Events.L3
+                             (prod InterpreterStackBigIntptr.LLVM.MEM.MMEP.MMSP.MemState
+                                (prod MemPropT.store_id (prod (prod InterpreterStackBigIntptr.LLVM.Local.local_env InterpreterStackBigIntptr.LLVM.Stack.lstack) (prod InterpreterStackBigIntptr.LLVM.Global.global_env InterpreterStackBigIntptr.LP.Events.DV.dvalue)))))
+                          (fun (t1 : dtyp) (f1 : uvalue) (args1 : list dvalue) =>
+                           @eq_rect Type dvalue
+                             (fun X1 : Type =>
+                              forall (_ : forall _ : X1, itree L3 (prod FinMem.MMEP.MMSP.MemState (prod MemPropT.store_id (prod (prod local_env (@stack local_env)) (prod global_env dvalue))))) (_ : ExternalCallE X1),
+                              itree InfLP.Events.L3
+                                (prod InterpreterStackBigIntptr.LLVM.MEM.MMEP.MMSP.MemState
+                                   (prod MemPropT.store_id (prod (prod InterpreterStackBigIntptr.LLVM.Local.local_env InterpreterStackBigIntptr.LLVM.Stack.lstack) (prod InterpreterStackBigIntptr.LLVM.Global.global_env InterpreterStackBigIntptr.LP.Events.DV.dvalue)))))
+                             (fun (k1 : forall _ : dvalue, itree L3 (prod FinMem.MMEP.MMSP.MemState (prod MemPropT.store_id (prod (prod local_env (@stack local_env)) (prod global_env dvalue))))) (_ : ExternalCallE dvalue) =>
+                              @go InfLP.Events.L3
+                                (prod InterpreterStackBigIntptr.LLVM.MEM.MMEP.MMSP.MemState
+                                   (prod MemPropT.store_id (prod (prod InterpreterStackBigIntptr.LLVM.Local.local_env InterpreterStackBigIntptr.LLVM.Stack.lstack) (prod InterpreterStackBigIntptr.LLVM.Global.global_env InterpreterStackBigIntptr.LP.Events.DV.dvalue))))
+                                (@VisF InfLP.Events.L3
+                                   (prod InterpreterStackBigIntptr.LLVM.MEM.MMEP.MMSP.MemState
+                                      (prod MemPropT.store_id (prod (prod InterpreterStackBigIntptr.LLVM.Local.local_env InterpreterStackBigIntptr.LLVM.Stack.lstack) (prod InterpreterStackBigIntptr.LLVM.Global.global_env InterpreterStackBigIntptr.LP.Events.DV.dvalue))))
+                                   (itree InfLP.Events.L3
+                                      (prod InterpreterStackBigIntptr.LLVM.MEM.MMEP.MMSP.MemState
+                                         (prod MemPropT.store_id (prod (prod InterpreterStackBigIntptr.LLVM.Local.local_env InterpreterStackBigIntptr.LLVM.Stack.lstack) (prod InterpreterStackBigIntptr.LLVM.Global.global_env InterpreterStackBigIntptr.LP.Events.DV.dvalue))))) E1.DV.dvalue
+                                   (@subevent E1.ExternalCallE InfLP.Events.L3
+                                      (@ReSum_inl (forall _ : Type, Type) IFun sum1 Cat_IFun Inl_sum1 E1.ExternalCallE InfLP.Events.ExternalCallE (sum1 InfLP.Events.PickUvalueE (sum1 OOME (sum1 UBE (sum1 DebugE FailureE)))) (@ReSum_id (forall _ : Type, Type) IFun Id_IFun InfLP.Events.ExternalCallE)) E1.DV.dvalue
+                                      (E1.ExternalCall t1 (fin_to_inf_uvalue f1) (@map LLVMParams64BitIntptr.Events.DV.dvalue LLVMParamsBigIntptr.Events.DV.dvalue fin_to_inf_dvalue args1)))
+                                   (fun x0 : E1.DV.dvalue =>
+                                    get_inf_tree
+                                      (let H5 : OOM DVCInfFin.DV2.dvalue := DVCInfFin.dvalue_convert_strict x0 in
+                                       match H5 return (itree L3 (prod FinMem.MMEP.MMSP.MemState (prod MemPropT.store_id (prod (prod local_env (@stack local_env)) (prod global_env dvalue))))) with
+                                       | NoOom a => (fun d : DVCInfFin.DV2.dvalue => k1 d) a
+                                       | Oom s =>
+                                           (fun s0 : string =>
+                                            @raiseOOM L3
+                                              (@ReSum_inr (forall _ : Type, Type) IFun sum1 Cat_IFun Inr_sum1 OOME (sum1 PickUvalueE (sum1 OOME (sum1 UBE (sum1 DebugE FailureE)))) ExternalCallE
+                                                 (@ReSum_inr (forall _ : Type, Type) IFun sum1 Cat_IFun Inr_sum1 OOME (sum1 OOME (sum1 UBE (sum1 DebugE FailureE))) PickUvalueE
+                                                    (@ReSum_inl (forall _ : Type, Type) IFun sum1 Cat_IFun Inl_sum1 OOME OOME (sum1 UBE (sum1 DebugE FailureE)) (@ReSum_id (forall _ : Type, Type) IFun Id_IFun OOME))))
+                                              (prod FinMem.MMEP.MMSP.MemState (prod MemPropT.store_id (prod (prod local_env (@stack local_env)) (prod global_env dvalue)))) s0) s
+                                       end)))) X0 H2 k0 H0) X0 H3) H1 t0 f0 args0) t f args
+                  end in
+                X1 (@eq_refl Type X0)) H) x
+          | inr1 x =>
+              (fun X1 : sum1 PickUvalueE (sum1 OOME (sum1 UBE (sum1 DebugE FailureE))) X0 =>
+               (fun X2 : sum1 PickUvalueE (sum1 OOME (sum1 UBE (sum1 DebugE FailureE))) X0 =>
+                let X3 :
+                  itree InfLP.Events.L3
+                    (prod InterpreterStackBigIntptr.LLVM.MEM.MMEP.MMSP.MemState (prod MemPropT.store_id (prod (prod InterpreterStackBigIntptr.LLVM.Local.local_env InterpreterStackBigIntptr.LLVM.Stack.lstack) (prod InterpreterStackBigIntptr.LLVM.Global.global_env InterpreterStackBigIntptr.LP.Events.DV.dvalue)))) :=
+                  match
+                    X2
+                    return
+                      (itree InfLP.Events.L3
+                         (prod InterpreterStackBigIntptr.LLVM.MEM.MMEP.MMSP.MemState
+                            (prod MemPropT.store_id (prod (prod InterpreterStackBigIntptr.LLVM.Local.local_env InterpreterStackBigIntptr.LLVM.Stack.lstack) (prod InterpreterStackBigIntptr.LLVM.Global.global_env InterpreterStackBigIntptr.LP.Events.DV.dvalue)))))
+                  with
+                  | inl1 x0 =>
+                      (fun X3 : PickUvalueE X0 =>
+                       (fun X4 : PickUvalueE X0 =>
+                        let X5 :
+                          forall _ : @eq Type X0 X0,
+                          itree InfLP.Events.L3
+                            (prod InterpreterStackBigIntptr.LLVM.MEM.MMEP.MMSP.MemState
+                               (prod MemPropT.store_id (prod (prod InterpreterStackBigIntptr.LLVM.Local.local_env InterpreterStackBigIntptr.LLVM.Stack.lstack) (prod InterpreterStackBigIntptr.LLVM.Global.global_env InterpreterStackBigIntptr.LP.Events.DV.dvalue)))) :=
+                          match
+                            X4 in (PickE T)
+                            return
+                              (forall _ : @eq Type T X0,
+                               itree InfLP.Events.L3
+                                 (prod InterpreterStackBigIntptr.LLVM.MEM.MMEP.MMSP.MemState
+                                    (prod MemPropT.store_id (prod (prod InterpreterStackBigIntptr.LLVM.Local.local_env InterpreterStackBigIntptr.LLVM.Stack.lstack) (prod InterpreterStackBigIntptr.LLVM.Global.global_env InterpreterStackBigIntptr.LP.Events.DV.dvalue)))))
+                          with
+                          | pick Pre x1 =>
+                              (fun (Pre0 : Prop) (x2 : uvalue) (H : @eq Type (@sig dvalue (fun _ : dvalue => True)) X0) =>
+                               (fun H0 : @eq Type (@sig dvalue (fun _ : dvalue => True)) X0 =>
+                                let H1 : @eq Type (@sig dvalue (fun _ : dvalue => True)) X0 := H0 in
+                                @eq_rect Type (@sig dvalue (fun _ : dvalue => True))
+                                  (fun _ : Type =>
+                                   forall (_ : Prop) (_ : uvalue),
+                                   itree InfLP.Events.L3
+                                     (prod InterpreterStackBigIntptr.LLVM.MEM.MMEP.MMSP.MemState
+                                        (prod MemPropT.store_id (prod (prod InterpreterStackBigIntptr.LLVM.Local.local_env InterpreterStackBigIntptr.LLVM.Stack.lstack) (prod InterpreterStackBigIntptr.LLVM.Global.global_env InterpreterStackBigIntptr.LP.Events.DV.dvalue)))))
+                                  (fun (Pre1 : Prop) (x3 : uvalue) =>
+                                   @eq_rect Type (@sig dvalue (fun _ : dvalue => True))
+                                     (fun X5 : Type =>
+                                      forall (_ : forall _ : X5, itree L3 (prod FinMem.MMEP.MMSP.MemState (prod MemPropT.store_id (prod (prod local_env (@stack local_env)) (prod global_env dvalue))))) (_ : PickUvalueE X5),
+                                      itree InfLP.Events.L3
+                                        (prod InterpreterStackBigIntptr.LLVM.MEM.MMEP.MMSP.MemState
+                                           (prod MemPropT.store_id (prod (prod InterpreterStackBigIntptr.LLVM.Local.local_env InterpreterStackBigIntptr.LLVM.Stack.lstack) (prod InterpreterStackBigIntptr.LLVM.Global.global_env InterpreterStackBigIntptr.LP.Events.DV.dvalue)))))
+                                     (fun (k1 : forall _ : @sig dvalue (fun _ : dvalue => True), itree L3 (prod FinMem.MMEP.MMSP.MemState (prod MemPropT.store_id (prod (prod local_env (@stack local_env)) (prod global_env dvalue))))) (_ : PickUvalueE (@sig dvalue (fun _ : dvalue => True))) =>
+                                      @go InfLP.Events.L3
+                                        (prod InterpreterStackBigIntptr.LLVM.MEM.MMEP.MMSP.MemState
+                                           (prod MemPropT.store_id (prod (prod InterpreterStackBigIntptr.LLVM.Local.local_env InterpreterStackBigIntptr.LLVM.Stack.lstack) (prod InterpreterStackBigIntptr.LLVM.Global.global_env InterpreterStackBigIntptr.LP.Events.DV.dvalue))))
+                                        (@VisF InfLP.Events.L3
+                                           (prod InterpreterStackBigIntptr.LLVM.MEM.MMEP.MMSP.MemState
+                                              (prod MemPropT.store_id (prod (prod InterpreterStackBigIntptr.LLVM.Local.local_env InterpreterStackBigIntptr.LLVM.Stack.lstack) (prod InterpreterStackBigIntptr.LLVM.Global.global_env InterpreterStackBigIntptr.LP.Events.DV.dvalue))))
+                                           (itree InfLP.Events.L3
+                                              (prod InterpreterStackBigIntptr.LLVM.MEM.MMEP.MMSP.MemState
+                                                 (prod MemPropT.store_id (prod (prod InterpreterStackBigIntptr.LLVM.Local.local_env InterpreterStackBigIntptr.LLVM.Stack.lstack) (prod InterpreterStackBigIntptr.LLVM.Global.global_env InterpreterStackBigIntptr.LP.Events.DV.dvalue)))))
+                                           (@sig InfLP.Events.DV.dvalue (fun _ : InfLP.Events.DV.dvalue => True))
+                                           (@subevent (@E1.PickE LLVMParamsBigIntptr.Events.DV.uvalue InfLP.Events.DV.dvalue (fun (_ : InfLP.Events.DV.uvalue) (_ : InfLP.Events.DV.dvalue) => True)) InfLP.Events.L3
+                                              (@ReSum_inr (forall _ : Type, Type) IFun sum1 Cat_IFun Inr_sum1 (@E1.PickE LLVMParamsBigIntptr.Events.DV.uvalue InfLP.Events.DV.dvalue (fun (_ : InfLP.Events.DV.uvalue) (_ : InfLP.Events.DV.dvalue) => True))
+                                                 (sum1 InfLP.Events.PickUvalueE (sum1 OOME (sum1 UBE (sum1 DebugE FailureE)))) InfLP.Events.ExternalCallE
+                                                 (@ReSum_inl (forall _ : Type, Type) IFun sum1 Cat_IFun Inl_sum1 (@E1.PickE LLVMParamsBigIntptr.Events.DV.uvalue InfLP.Events.DV.dvalue (fun (_ : InfLP.Events.DV.uvalue) (_ : InfLP.Events.DV.dvalue) => True)) InfLP.Events.PickUvalueE
+                                                    (sum1 OOME (sum1 UBE (sum1 DebugE FailureE))) (@ReSum_id (forall _ : Type, Type) IFun Id_IFun InfLP.Events.PickUvalueE))) (@sig InfLP.Events.DV.dvalue (fun _ : InfLP.Events.DV.dvalue => True))
+                                              (@E1.pick LLVMParamsBigIntptr.Events.DV.uvalue InfLP.Events.DV.dvalue (fun (_ : InfLP.Events.DV.uvalue) (_ : InfLP.Events.DV.dvalue) => True) Pre1 (fin_to_inf_uvalue x3)))
+                                           (fun res : @sig InfLP.Events.DV.dvalue (fun _ : InfLP.Events.DV.dvalue => True) =>
+                                            match
+                                              res
+                                              return
+                                                (itree InfLP.Events.L3
+                                                   (prod InterpreterStackBigIntptr.LLVM.MEM.MMEP.MMSP.MemState
+                                                      (prod MemPropT.store_id (prod (prod InterpreterStackBigIntptr.LLVM.Local.local_env InterpreterStackBigIntptr.LLVM.Stack.lstack) (prod InterpreterStackBigIntptr.LLVM.Global.global_env InterpreterStackBigIntptr.LP.Events.DV.dvalue)))))
+                                            with
+                                            | @exist _ _ x4 p =>
+                                                (fun (x5 : InfLP.Events.DV.dvalue) (t : True) =>
+                                                 get_inf_tree
+                                                   (let H2 : OOM DVCInfFin.DV2.dvalue := DVCInfFin.dvalue_convert_strict x5 in
+                                                    match H2 return (itree L3 (prod FinMem.MMEP.MMSP.MemState (prod MemPropT.store_id (prod (prod local_env (@stack local_env)) (prod global_env dvalue))))) with
+                                                    | NoOom a => (fun d : DVCInfFin.DV2.dvalue => k1 (@exist dvalue (fun _ : dvalue => True) d t)) a
+                                                    | Oom s =>
+                                                        (fun s0 : string =>
+                                                         @raiseOOM L3
+                                                           (@ReSum_inr (forall _ : Type, Type) IFun sum1 Cat_IFun Inr_sum1 OOME (sum1 PickUvalueE (sum1 OOME (sum1 UBE (sum1 DebugE FailureE)))) ExternalCallE
+                                                              (@ReSum_inr (forall _ : Type, Type) IFun sum1 Cat_IFun Inr_sum1 OOME (sum1 OOME (sum1 UBE (sum1 DebugE FailureE))) PickUvalueE
+                                                                 (@ReSum_inl (forall _ : Type, Type) IFun sum1 Cat_IFun Inl_sum1 OOME OOME (sum1 UBE (sum1 DebugE FailureE)) (@ReSum_id (forall _ : Type, Type) IFun Id_IFun OOME))))
+                                                           (prod FinMem.MMEP.MMSP.MemState (prod MemPropT.store_id (prod (prod local_env (@stack local_env)) (prod global_env dvalue)))) s0) s
+                                                    end)) x4 p
+                                            end))) X0 H0 k0 X4) X0 H1) H Pre0 x2) Pre x1
+                          end in
+                        X5 (@eq_refl Type X0)) X3) x0
+                  | inr1 x0 =>
+                      (fun H : sum1 OOME (sum1 UBE (sum1 DebugE FailureE)) X0 =>
+                       (fun H0 : sum1 OOME (sum1 UBE (sum1 DebugE FailureE)) X0 =>
+                        let X3 :
+                          itree InfLP.Events.L3
+                            (prod InterpreterStackBigIntptr.LLVM.MEM.MMEP.MMSP.MemState
+                               (prod MemPropT.store_id (prod (prod InterpreterStackBigIntptr.LLVM.Local.local_env InterpreterStackBigIntptr.LLVM.Stack.lstack) (prod InterpreterStackBigIntptr.LLVM.Global.global_env InterpreterStackBigIntptr.LP.Events.DV.dvalue)))) :=
+                          match
+                            H0
+                            return
+                              (itree InfLP.Events.L3
+                                 (prod InterpreterStackBigIntptr.LLVM.MEM.MMEP.MMSP.MemState
+                                    (prod MemPropT.store_id (prod (prod InterpreterStackBigIntptr.LLVM.Local.local_env InterpreterStackBigIntptr.LLVM.Stack.lstack) (prod InterpreterStackBigIntptr.LLVM.Global.global_env InterpreterStackBigIntptr.LP.Events.DV.dvalue)))))
+                          with
+                          | inl1 x1 =>
+                              (fun H1 : OOME X0 =>
+                               (fun H2 : OOME X0 =>
+                                let X3 :
+                                  forall _ : @eq Type X0 X0,
+                                  itree InfLP.Events.L3
+                                    (prod InterpreterStackBigIntptr.LLVM.MEM.MMEP.MMSP.MemState
+                                       (prod MemPropT.store_id (prod (prod InterpreterStackBigIntptr.LLVM.Local.local_env InterpreterStackBigIntptr.LLVM.Stack.lstack) (prod InterpreterStackBigIntptr.LLVM.Global.global_env InterpreterStackBigIntptr.LP.Events.DV.dvalue)))) :=
+                                  match
+                                    H2 in (OOME T)
+                                    return
+                                      (forall _ : @eq Type T X0,
+                                       itree InfLP.Events.L3
+                                         (prod InterpreterStackBigIntptr.LLVM.MEM.MMEP.MMSP.MemState
+                                            (prod MemPropT.store_id (prod (prod InterpreterStackBigIntptr.LLVM.Local.local_env InterpreterStackBigIntptr.LLVM.Stack.lstack) (prod InterpreterStackBigIntptr.LLVM.Global.global_env InterpreterStackBigIntptr.LP.Events.DV.dvalue)))))
+                                  with
+                                  | ThrowOOM x2 =>
+                                      (fun (H3 : string) (H4 : @eq Type Empty_set X0) =>
+                                       (fun H5 : @eq Type Empty_set X0 =>
+                                        let H6 : @eq Type Empty_set X0 := H5 in
+                                        @eq_rect Type Empty_set
+                                          (fun _ : Type =>
+                                           forall _ : string,
+                                           itree InfLP.Events.L3
+                                             (prod InterpreterStackBigIntptr.LLVM.MEM.MMEP.MMSP.MemState
+                                                (prod MemPropT.store_id (prod (prod InterpreterStackBigIntptr.LLVM.Local.local_env InterpreterStackBigIntptr.LLVM.Stack.lstack) (prod InterpreterStackBigIntptr.LLVM.Global.global_env InterpreterStackBigIntptr.LP.Events.DV.dvalue)))))
+                                          (fun H7 : string =>
+                                           @eq_rect Type Empty_set
+                                             (fun X3 : Type =>
+                                              forall (_ : forall _ : X3, itree L3 (prod FinMem.MMEP.MMSP.MemState (prod MemPropT.store_id (prod (prod local_env (@stack local_env)) (prod global_env dvalue))))) (_ : OOME X3),
+                                              itree InfLP.Events.L3
+                                                (prod InterpreterStackBigIntptr.LLVM.MEM.MMEP.MMSP.MemState
+                                                   (prod MemPropT.store_id (prod (prod InterpreterStackBigIntptr.LLVM.Local.local_env InterpreterStackBigIntptr.LLVM.Stack.lstack) (prod InterpreterStackBigIntptr.LLVM.Global.global_env InterpreterStackBigIntptr.LP.Events.DV.dvalue)))))
+                                             (fun (_ : forall _ : Empty_set, itree L3 (prod FinMem.MMEP.MMSP.MemState (prod MemPropT.store_id (prod (prod local_env (@stack local_env)) (prod global_env dvalue))))) (_ : OOME Empty_set) =>
+                                              @raiseOOM InfLP.Events.L3
+                                                (@ReSum_inr (forall _ : Type, Type) IFun sum1 Cat_IFun Inr_sum1 OOME (sum1 InfLP.Events.PickUvalueE (sum1 OOME (sum1 UBE (sum1 DebugE FailureE)))) InfLP.Events.ExternalCallE
+                                                   (@ReSum_inr (forall _ : Type, Type) IFun sum1 Cat_IFun Inr_sum1 OOME (sum1 OOME (sum1 UBE (sum1 DebugE FailureE))) InfLP.Events.PickUvalueE
+                                                      (@ReSum_inl (forall _ : Type, Type) IFun sum1 Cat_IFun Inl_sum1 OOME OOME (sum1 UBE (sum1 DebugE FailureE)) (@ReSum_id (forall _ : Type, Type) IFun Id_IFun OOME))))
+                                                (prod InterpreterStackBigIntptr.LLVM.MEM.MMEP.MMSP.MemState
+                                                   (prod MemPropT.store_id (prod (prod InterpreterStackBigIntptr.LLVM.Local.local_env InterpreterStackBigIntptr.LLVM.Stack.lstack) (prod InterpreterStackBigIntptr.LLVM.Global.global_env InterpreterStackBigIntptr.LP.Events.DV.dvalue)))) H7) X0 H5 k0 H2) X0 H6) H4 H3)
+                                        x2
+                                  end in
+                                X3 (@eq_refl Type X0)) H1) x1
+                          | inr1 x1 =>
+                              (fun H1 : sum1 UBE (sum1 DebugE FailureE) X0 =>
+                               (fun H2 : sum1 UBE (sum1 DebugE FailureE) X0 =>
+                                let X3 :
+                                  itree InfLP.Events.L3
+                                    (prod InterpreterStackBigIntptr.LLVM.MEM.MMEP.MMSP.MemState
+                                       (prod MemPropT.store_id (prod (prod InterpreterStackBigIntptr.LLVM.Local.local_env InterpreterStackBigIntptr.LLVM.Stack.lstack) (prod InterpreterStackBigIntptr.LLVM.Global.global_env InterpreterStackBigIntptr.LP.Events.DV.dvalue)))) :=
+                                  match
+                                    H2
+                                    return
+                                      (itree InfLP.Events.L3
+                                         (prod InterpreterStackBigIntptr.LLVM.MEM.MMEP.MMSP.MemState
+                                            (prod MemPropT.store_id (prod (prod InterpreterStackBigIntptr.LLVM.Local.local_env InterpreterStackBigIntptr.LLVM.Stack.lstack) (prod InterpreterStackBigIntptr.LLVM.Global.global_env InterpreterStackBigIntptr.LP.Events.DV.dvalue)))))
+                                  with
+                                  | inl1 x2 =>
+                                      (fun H3 : UBE X0 =>
+                                       (fun H4 : UBE X0 =>
+                                        let X3 :
+                                          forall _ : @eq Type X0 X0,
+                                          itree InfLP.Events.L3
+                                            (prod InterpreterStackBigIntptr.LLVM.MEM.MMEP.MMSP.MemState
+                                               (prod MemPropT.store_id (prod (prod InterpreterStackBigIntptr.LLVM.Local.local_env InterpreterStackBigIntptr.LLVM.Stack.lstack) (prod InterpreterStackBigIntptr.LLVM.Global.global_env InterpreterStackBigIntptr.LP.Events.DV.dvalue)))) :=
+                                          match
+                                            H4 in (UBE T)
+                                            return
+                                              (forall _ : @eq Type T X0,
+                                               itree InfLP.Events.L3
+                                                 (prod InterpreterStackBigIntptr.LLVM.MEM.MMEP.MMSP.MemState
+                                                    (prod MemPropT.store_id (prod (prod InterpreterStackBigIntptr.LLVM.Local.local_env InterpreterStackBigIntptr.LLVM.Stack.lstack) (prod InterpreterStackBigIntptr.LLVM.Global.global_env InterpreterStackBigIntptr.LP.Events.DV.dvalue)))))
+                                          with
+                                          | ThrowUB x3 =>
+                                              (fun (H5 : string) (H6 : @eq Type Empty_set X0) =>
+                                               (fun H7 : @eq Type Empty_set X0 =>
+                                                let H8 : @eq Type Empty_set X0 := H7 in
+                                                @eq_rect Type Empty_set
+                                                  (fun _ : Type =>
+                                                   forall _ : string,
+                                                   itree InfLP.Events.L3
+                                                     (prod InterpreterStackBigIntptr.LLVM.MEM.MMEP.MMSP.MemState
+                                                        (prod MemPropT.store_id (prod (prod InterpreterStackBigIntptr.LLVM.Local.local_env InterpreterStackBigIntptr.LLVM.Stack.lstack) (prod InterpreterStackBigIntptr.LLVM.Global.global_env InterpreterStackBigIntptr.LP.Events.DV.dvalue)))))
+                                                  (fun H9 : string =>
+                                                   @eq_rect Type Empty_set
+                                                     (fun X3 : Type =>
+                                                      forall (_ : forall _ : X3, itree L3 (prod FinMem.MMEP.MMSP.MemState (prod MemPropT.store_id (prod (prod local_env (@stack local_env)) (prod global_env dvalue))))) (_ : UBE X3),
+                                                      itree InfLP.Events.L3
+                                                        (prod InterpreterStackBigIntptr.LLVM.MEM.MMEP.MMSP.MemState
+                                                           (prod MemPropT.store_id (prod (prod InterpreterStackBigIntptr.LLVM.Local.local_env InterpreterStackBigIntptr.LLVM.Stack.lstack) (prod InterpreterStackBigIntptr.LLVM.Global.global_env InterpreterStackBigIntptr.LP.Events.DV.dvalue)))))
+                                                     (fun (_ : forall _ : Empty_set, itree L3 (prod FinMem.MMEP.MMSP.MemState (prod MemPropT.store_id (prod (prod local_env (@stack local_env)) (prod global_env dvalue))))) (_ : UBE Empty_set) =>
+                                                      @raiseUB InfLP.Events.L3
+                                                        (@ReSum_inr (forall _ : Type, Type) IFun sum1 Cat_IFun Inr_sum1 UBE (sum1 InfLP.Events.PickUvalueE (sum1 OOME (sum1 UBE (sum1 DebugE FailureE)))) InfLP.Events.ExternalCallE
+                                                           (@ReSum_inr (forall _ : Type, Type) IFun sum1 Cat_IFun Inr_sum1 UBE (sum1 OOME (sum1 UBE (sum1 DebugE FailureE))) InfLP.Events.PickUvalueE
+                                                              (@ReSum_inr (forall _ : Type, Type) IFun sum1 Cat_IFun Inr_sum1 UBE (sum1 UBE (sum1 DebugE FailureE)) OOME
+                                                                 (@ReSum_inl (forall _ : Type, Type) IFun sum1 Cat_IFun Inl_sum1 UBE UBE (sum1 DebugE FailureE) (@ReSum_id (forall _ : Type, Type) IFun Id_IFun UBE)))))
+                                                        (prod InterpreterStackBigIntptr.LLVM.MEM.MMEP.MMSP.MemState
+                                                           (prod MemPropT.store_id (prod (prod InterpreterStackBigIntptr.LLVM.Local.local_env InterpreterStackBigIntptr.LLVM.Stack.lstack) (prod InterpreterStackBigIntptr.LLVM.Global.global_env InterpreterStackBigIntptr.LP.Events.DV.dvalue)))) H9) X0 H7 k0 H4) X0 H8)
+                                                 H6 H5) x3
+                                          end in
+                                        X3 (@eq_refl Type X0)) H3) x2
+                                  | inr1 x2 =>
+                                      (fun H3 : sum1 DebugE FailureE X0 =>
+                                       (fun H4 : sum1 DebugE FailureE X0 =>
+                                        let X3 :
+                                          itree InfLP.Events.L3
+                                            (prod InterpreterStackBigIntptr.LLVM.MEM.MMEP.MMSP.MemState
+                                               (prod MemPropT.store_id (prod (prod InterpreterStackBigIntptr.LLVM.Local.local_env InterpreterStackBigIntptr.LLVM.Stack.lstack) (prod InterpreterStackBigIntptr.LLVM.Global.global_env InterpreterStackBigIntptr.LP.Events.DV.dvalue)))) :=
+                                          match
+                                            H4
+                                            return
+                                              (itree InfLP.Events.L3
+                                                 (prod InterpreterStackBigIntptr.LLVM.MEM.MMEP.MMSP.MemState
+                                                    (prod MemPropT.store_id (prod (prod InterpreterStackBigIntptr.LLVM.Local.local_env InterpreterStackBigIntptr.LLVM.Stack.lstack) (prod InterpreterStackBigIntptr.LLVM.Global.global_env InterpreterStackBigIntptr.LP.Events.DV.dvalue)))))
+                                          with
+                                          | inl1 x3 =>
+                                              (fun H5 : DebugE X0 =>
+                                               (fun H6 : DebugE X0 =>
+                                                let X3 :
+                                                  forall _ : @eq Type X0 X0,
+                                                  itree InfLP.Events.L3
+                                                    (prod InterpreterStackBigIntptr.LLVM.MEM.MMEP.MMSP.MemState
+                                                       (prod MemPropT.store_id (prod (prod InterpreterStackBigIntptr.LLVM.Local.local_env InterpreterStackBigIntptr.LLVM.Stack.lstack) (prod InterpreterStackBigIntptr.LLVM.Global.global_env InterpreterStackBigIntptr.LP.Events.DV.dvalue)))) :=
+                                                  match
+                                                    H6 in (DebugE T)
+                                                    return
+                                                      (forall _ : @eq Type T X0,
+                                                       itree InfLP.Events.L3
+                                                         (prod InterpreterStackBigIntptr.LLVM.MEM.MMEP.MMSP.MemState
+                                                            (prod MemPropT.store_id (prod (prod InterpreterStackBigIntptr.LLVM.Local.local_env InterpreterStackBigIntptr.LLVM.Stack.lstack) (prod InterpreterStackBigIntptr.LLVM.Global.global_env InterpreterStackBigIntptr.LP.Events.DV.dvalue)))))
+                                                  with
+                                                  | Debug x4 =>
+                                                      (fun (H7 : string) (H8 : @eq Type unit X0) =>
+                                                       (fun H9 : @eq Type unit X0 =>
+                                                        let H10 : @eq Type unit X0 := H9 in
+                                                        @eq_rect Type unit
+                                                          (fun _ : Type =>
+                                                           forall _ : string,
+                                                           itree InfLP.Events.L3
+                                                             (prod InterpreterStackBigIntptr.LLVM.MEM.MMEP.MMSP.MemState
+                                                                (prod MemPropT.store_id (prod (prod InterpreterStackBigIntptr.LLVM.Local.local_env InterpreterStackBigIntptr.LLVM.Stack.lstack) (prod InterpreterStackBigIntptr.LLVM.Global.global_env InterpreterStackBigIntptr.LP.Events.DV.dvalue)))))
+                                                          (fun H11 : string =>
+                                                           @eq_rect Type unit
+                                                             (fun X3 : Type =>
+                                                              forall (_ : forall _ : X3, itree L3 (prod FinMem.MMEP.MMSP.MemState (prod MemPropT.store_id (prod (prod local_env (@stack local_env)) (prod global_env dvalue))))) (_ : DebugE X3),
+                                                              itree InfLP.Events.L3
+                                                                (prod InterpreterStackBigIntptr.LLVM.MEM.MMEP.MMSP.MemState
+                                                                   (prod MemPropT.store_id (prod (prod InterpreterStackBigIntptr.LLVM.Local.local_env InterpreterStackBigIntptr.LLVM.Stack.lstack) (prod InterpreterStackBigIntptr.LLVM.Global.global_env InterpreterStackBigIntptr.LP.Events.DV.dvalue)))))
+                                                             (fun (k1 : forall _ : unit, itree L3 (prod FinMem.MMEP.MMSP.MemState (prod MemPropT.store_id (prod (prod local_env (@stack local_env)) (prod global_env dvalue))))) (_ : DebugE unit) =>
+                                                              @go InfLP.Events.L3
+                                                                (prod InterpreterStackBigIntptr.LLVM.MEM.MMEP.MMSP.MemState
+                                                                   (prod MemPropT.store_id (prod (prod InterpreterStackBigIntptr.LLVM.Local.local_env InterpreterStackBigIntptr.LLVM.Stack.lstack) (prod InterpreterStackBigIntptr.LLVM.Global.global_env InterpreterStackBigIntptr.LP.Events.DV.dvalue))))
+                                                                (@VisF InfLP.Events.L3
+                                                                   (prod InterpreterStackBigIntptr.LLVM.MEM.MMEP.MMSP.MemState
+                                                                      (prod MemPropT.store_id (prod (prod InterpreterStackBigIntptr.LLVM.Local.local_env InterpreterStackBigIntptr.LLVM.Stack.lstack) (prod InterpreterStackBigIntptr.LLVM.Global.global_env InterpreterStackBigIntptr.LP.Events.DV.dvalue))))
+                                                                   (itree InfLP.Events.L3
+                                                                      (prod InterpreterStackBigIntptr.LLVM.MEM.MMEP.MMSP.MemState
+                                                                         (prod MemPropT.store_id (prod (prod InterpreterStackBigIntptr.LLVM.Local.local_env InterpreterStackBigIntptr.LLVM.Stack.lstack) (prod InterpreterStackBigIntptr.LLVM.Global.global_env InterpreterStackBigIntptr.LP.Events.DV.dvalue))))) unit
+                                                                   (@subevent DebugE InfLP.Events.L3
+                                                                      (@ReSum_inr (forall _ : Type, Type) IFun sum1 Cat_IFun Inr_sum1 DebugE (sum1 InfLP.Events.PickUvalueE (sum1 OOME (sum1 UBE (sum1 DebugE FailureE)))) InfLP.Events.ExternalCallE
+                                                                         (@ReSum_inr (forall _ : Type, Type) IFun sum1 Cat_IFun Inr_sum1 DebugE (sum1 OOME (sum1 UBE (sum1 DebugE FailureE))) InfLP.Events.PickUvalueE
+                                                                            (@ReSum_inr (forall _ : Type, Type) IFun sum1 Cat_IFun Inr_sum1 DebugE (sum1 UBE (sum1 DebugE FailureE)) OOME
+                                                                               (@ReSum_inr (forall _ : Type, Type) IFun sum1 Cat_IFun Inr_sum1 DebugE (sum1 DebugE FailureE) UBE
+                                                                                  (@ReSum_inl (forall _ : Type, Type) IFun sum1 Cat_IFun Inl_sum1 DebugE DebugE FailureE (@ReSum_id (forall _ : Type, Type) IFun Id_IFun DebugE)))))) unit (Debug H11)) (fun H13 : unit => get_inf_tree (k1 H13)))) X0 H9 k0 H6) X0 H10) H8 H7) x4
+                                                  end in
+                                                X3 (@eq_refl Type X0)) H5) x3
+                                          | inr1 x3 =>
+                                              (fun H5 : FailureE X0 =>
+                                               (fun H6 : FailureE X0 =>
+                                                let X3 :
+                                                  forall _ : @eq Type X0 X0,
+                                                  itree InfLP.Events.L3
+                                                    (prod InterpreterStackBigIntptr.LLVM.MEM.MMEP.MMSP.MemState
+                                                       (prod MemPropT.store_id (prod (prod InterpreterStackBigIntptr.LLVM.Local.local_env InterpreterStackBigIntptr.LLVM.Stack.lstack) (prod InterpreterStackBigIntptr.LLVM.Global.global_env InterpreterStackBigIntptr.LP.Events.DV.dvalue)))) :=
+                                                  match
+                                                    H6 in (FailureE T)
+                                                    return
+                                                      (forall _ : @eq Type T X0,
+                                                       itree InfLP.Events.L3
+                                                         (prod InterpreterStackBigIntptr.LLVM.MEM.MMEP.MMSP.MemState
+                                                            (prod MemPropT.store_id (prod (prod InterpreterStackBigIntptr.LLVM.Local.local_env InterpreterStackBigIntptr.LLVM.Stack.lstack) (prod InterpreterStackBigIntptr.LLVM.Global.global_env InterpreterStackBigIntptr.LP.Events.DV.dvalue)))))
+                                                  with
+                                                  | Throw x4 =>
+                                                      (fun (H7 : string) (H8 : @eq Type Empty_set X0) =>
+                                                       (fun H9 : @eq Type Empty_set X0 =>
+                                                        let H10 : @eq Type Empty_set X0 := H9 in
+                                                        @eq_rect Type Empty_set
+                                                          (fun _ : Type =>
+                                                           forall _ : string,
+                                                           itree InfLP.Events.L3
+                                                             (prod InterpreterStackBigIntptr.LLVM.MEM.MMEP.MMSP.MemState
+                                                                (prod MemPropT.store_id (prod (prod InterpreterStackBigIntptr.LLVM.Local.local_env InterpreterStackBigIntptr.LLVM.Stack.lstack) (prod InterpreterStackBigIntptr.LLVM.Global.global_env InterpreterStackBigIntptr.LP.Events.DV.dvalue)))))
+                                                          (fun H11 : string =>
+                                                           @eq_rect Type Empty_set
+                                                             (fun X3 : Type =>
+                                                              forall (_ : forall _ : X3, itree L3 (prod FinMem.MMEP.MMSP.MemState (prod MemPropT.store_id (prod (prod local_env (@stack local_env)) (prod global_env dvalue))))) (_ : FailureE X3),
+                                                              itree InfLP.Events.L3
+                                                                (prod InterpreterStackBigIntptr.LLVM.MEM.MMEP.MMSP.MemState
+                                                                   (prod MemPropT.store_id (prod (prod InterpreterStackBigIntptr.LLVM.Local.local_env InterpreterStackBigIntptr.LLVM.Stack.lstack) (prod InterpreterStackBigIntptr.LLVM.Global.global_env InterpreterStackBigIntptr.LP.Events.DV.dvalue)))))
+                                                             (fun (_ : forall _ : Empty_set, itree L3 (prod FinMem.MMEP.MMSP.MemState (prod MemPropT.store_id (prod (prod local_env (@stack local_env)) (prod global_env dvalue))))) (_ : FailureE Empty_set) =>
+                                                              @LLVMEvents.raise InfLP.Events.L3
+                                                                (prod InterpreterStackBigIntptr.LLVM.MEM.MMEP.MMSP.MemState
+                                                                   (prod MemPropT.store_id (prod (prod InterpreterStackBigIntptr.LLVM.Local.local_env InterpreterStackBigIntptr.LLVM.Stack.lstack) (prod InterpreterStackBigIntptr.LLVM.Global.global_env InterpreterStackBigIntptr.LP.Events.DV.dvalue))))
+                                                                (@ReSum_inr (forall _ : Type, Type) IFun sum1 Cat_IFun Inr_sum1 FailureE (sum1 InfLP.Events.PickUvalueE (sum1 OOME (sum1 UBE (sum1 DebugE FailureE)))) InfLP.Events.ExternalCallE
+                                                                   (@ReSum_inr (forall _ : Type, Type) IFun sum1 Cat_IFun Inr_sum1 FailureE (sum1 OOME (sum1 UBE (sum1 DebugE FailureE))) InfLP.Events.PickUvalueE
+                                                                      (@ReSum_inr (forall _ : Type, Type) IFun sum1 Cat_IFun Inr_sum1 FailureE (sum1 UBE (sum1 DebugE FailureE)) OOME
+                                                                         (@ReSum_inr (forall _ : Type, Type) IFun sum1 Cat_IFun Inr_sum1 FailureE (sum1 DebugE FailureE) UBE
+                                                                            (@ReSum_inr (forall _ : Type, Type) IFun sum1 Cat_IFun Inr_sum1 FailureE FailureE DebugE (@ReSum_id (forall _ : Type, Type) IFun Id_IFun FailureE)))))) H11) X0 H9 k0 H6) X0 H10) H8 H7) x4
+                                                  end in
+                                                X3 (@eq_refl Type X0)) H5) x3
+                                          end in
+                                        X3) H3) x2
+                                  end in
+                                X3) H1) x1
+                          end in
+                        X3) H) x0
+                  end in
+                X3) X1) x
+          end in
+        X1) X e k
+    end.
+
+  Require Import ITree.Eq.EuttExtras.
+
+  Lemma paco2_eq_itree_refl : forall E R r (t : itree E R), paco2 (eqit_ eq false false id) r t t.
+  Proof.
+    intros. eapply paco2_mon with (r := bot2); intuition.
+    enough (t ≅ t); auto. reflexivity.
+  Qed.
+
+  Lemma get_inf_tree_equation :
+    forall t_fin2,
+      get_inf_tree t_fin2 ≅ _get_inf_tree (observe t_fin2).
+  Proof.
+    pcofix CIH.
+    intros t_fin2.
+    destruct (observe t_fin2) eqn:HTFIN.
+    - rewrite (itree_eta_ t_fin2).
+      rewrite HTFIN.
+      cbn.
+      pstep; red; cbn.
+      constructor.
+      reflexivity.
+    - rewrite (itree_eta_ t_fin2).
+      rewrite HTFIN.
+      cbn.
+      pstep; red; cbn.
+      constructor.
+      left.
+      apply paco2_eq_itree_refl.
+    - rewrite (itree_eta_ t_fin2).
+      unfold _get_inf_tree.
+      rewrite HTFIN.
+      destruct e.
+      admit.
+      admit.
+  Admitted.
 
   Lemma fin_to_inf_dvalue_refine_strict :
     forall d,
@@ -1002,6 +1973,79 @@ Module InfiniteToFinite.
           - admit.
         Admitted.
 
+        (* TODO: a little unsure of this one, but it seems plausible. *)
+        Set Nested Proofs Allowed.
+        Lemma fin_to_inf_uvalue_refine_strict' :
+          forall d_inf d_fin,
+            DVC1.uvalue_refine_strict d_inf d_fin ->
+            d_inf = fin_to_inf_uvalue d_fin.
+        Proof.
+          intros d_inf d_fin H.
+          rewrite DVC1.uvalue_refine_strict_equation in H.
+          unfold fin_to_inf_uvalue.
+          break_match; cbn in *.
+          destruct p.
+          clear Heqs.
+
+          induction d_inf;
+            try solve
+              [ rewrite DVC1.uvalue_convert_strict_equation in H;
+                cbn in *; inv H;
+                rewrite DVC2.uvalue_convert_strict_equation in e;
+                cbn in *; inv e;
+                auto
+              ].
+          - rewrite DVC1.uvalue_convert_strict_equation in H.
+            cbn in *.
+            break_match_hyp; inv H.
+            rewrite DVC2.uvalue_convert_strict_equation in e.
+            cbn in *.
+            break_match_hyp; inv e.
+            rewrite DVC1.uvalue_convert_strict_equation in e0.
+            cbn in *.
+            break_match_hyp; inv e0.
+
+            pose proof InfToFinAddrConvert.addr_convert_injective a a1 a0 Heqo Heqo1.
+            subst.
+            auto.
+          - rewrite DVC1.uvalue_convert_strict_equation in H.
+            cbn in *; break_match_hyp; inv H.
+            rewrite DVC2.uvalue_convert_strict_equation in e.
+            cbn in *; inv e.
+            rewrite DVC1.uvalue_convert_strict_equation in e0.
+            cbn in *; break_match_hyp; inv e0.
+            admit. (* Some painful IP / BigIP reasoning *)
+          - rewrite DVC1.uvalue_convert_strict_equation in H.
+            cbn in *; break_match_hyp; inv H.
+            rewrite DVC2.uvalue_convert_strict_equation in e.
+            cbn in *; break_match_hyp; inv e.
+            rewrite DVC1.uvalue_convert_strict_equation in e0.
+            cbn in *; break_match_hyp; inv e0.
+
+            induction fields.
+            + cbn in *. inv Heqo.
+              cbn in *. inv Heqo0.
+              reflexivity.
+            + rewrite map_monad_InT_unfold in Heqo.
+              cbn in *.
+              break_match_hyp; inv Heqo.
+              break_match_hyp; inv H1.
+
+              rewrite map_monad_InT_unfold in Heqo0.
+              cbn in *.
+              break_match_hyp; inv Heqo0.
+              break_match_hyp; inv H1.
+
+              rewrite map_monad_InT_unfold in Heqo1.
+              cbn in *.
+              break_match_hyp; inv Heqo1.
+              break_match_hyp; inv H1.
+              admit.
+          - admit.
+          - admit.
+          - admit.
+        Admitted.
+
         apply fin_to_inf_dvalue_refine_strict'; auto.
     - punfold RUN.
       red in RUN.
@@ -1114,9 +2158,287 @@ Module InfiniteToFinite.
               constructor.
               intros [] _.
            ++ specialize (EQ t0); contradiction.
-        -- { dependent induction RUN; subst.
+        -- { rewrite itree_eta in H1.
+             genobs t2 ot2.
+             clear t2 Heqot2.
+             dependent induction RUN; subst.
              - specialize (EQ t2).
                contradiction.
+             - pclearbot.
+               apply orutt_inv_Vis_r in H.
+               destruct H as [[U1 [e1 [k3 [M1 [EV_REL K_RUTT]]]]] | OOM].
+               2: {
+                 destruct OOM as [o OOM].
+                 inv OOM.
+                 repeat red in H0.
+                 rewrite H0 in H1.
+                 setoid_rewrite bind_trigger in H1.
+                 setoid_rewrite bind_vis in H1.
+                 punfold H1; red in H1; cbn in H1.
+                 dependent induction H1.
+                 - destruct o.
+                   eapply Interp_Memory_PropT_Vis_OOM.
+                   rewrite get_inf_tree_equation.
+                   cbn.
+                   unfold raiseOOM.
+                   rewrite bind_trigger.
+                   reflexivity.
+                 - specialize (EQ t1). contradiction.
+               }
+
+               repeat red in H0.
+               destruct e; cbn in *.
+               + red in H0.
+                 setoid_rewrite bind_trigger in H0.
+                 setoid_rewrite H0 in H1.
+                 setoid_rewrite bind_vis in H1.
+                 punfold H1; red in H1; cbn in H1.
+                 dependent induction H1.
+                 * {
+                     punfold M1; red in M1; cbn in M1.
+                     genobs m1 om1.
+                     dependent induction M1.
+                     - repeat red in EV_REL.
+                       destruct e1; repeat destruct s; repeat destruct i; try contradiction.
+                       destruct e0, e.
+                       destruct EV_REL as (T&F&ARGS); subst.
+                       eapply Interp_Memory_PropT_Vis with
+                         (k2:=
+                            fun '(_, (_, v)) => (get_inf_tree
+                               match DVCInfFin.dvalue_convert_strict v with
+                               | NoOom a => k0 a
+                               | Oom s => raiseOOM s
+                               end)
+                         ).
+                       + intros a b H H1 H2.
+                         admit.
+                       + cbn. red.
+                         setoid_rewrite bind_trigger.
+                         reflexivity.
+                       + rewrite get_inf_tree_equation.
+                         cbn.
+                         rewrite bind_vis.
+                         pose proof (fin_to_inf_uvalue_refine_strict' _ _ F).
+                         rewrite <- H.
+
+                         (* TODO: move this *)
+                         Lemma Forall2_map_eq :
+                           forall {A B} (f : A -> B) l1 l2,
+                             Forall2 (fun a b => f a = b) l1 l2 ->
+                             map f l1 = l2.
+                         Proof.
+                           intros A B f l1 l2 ALL.
+                           induction ALL; auto.
+                           rewrite map_cons.
+                           congruence.
+                         Qed.
+
+                         (* TODO: move this *)
+                         Lemma Forall2_flip :
+                           forall {A B} (P : A -> B -> Prop) l1 l2,
+                             Forall2 P l1 l2 <-> Forall2 (flip P) l2 l1.
+                         Proof.
+                           intros A B f l1 l2.
+                           split; intros ALL;
+                             induction ALL; auto.
+                         Qed.
+
+                         rewrite Forall2_map_eq with (l2:=args).
+                         2: {
+                           eapply Forall2_flip.
+                           eapply Util.Forall2_impl; [| apply ARGS].
+                           intros a b H1.
+                           red.
+                           symmetry.
+                           apply fin_to_inf_dvalue_refine_strict'.
+                           auto.
+                         }
+
+                         setoid_rewrite bind_ret_l.
+
+                         pstep; red; cbn.
+                         constructor.
+                         intros v. red.
+                         left.
+                         apply paco2_eqit_refl.
+
+
+                         unfold fin_to_inf_uvalue.
+                         rewrite DVCInfFin.uvalue_refine_strict_equation in F.
+                         destruct (uvalue_convert_strict_safe f0) as (f0'&CONV1&CONV2).
+                         rewrite <- F in CONV2.
+                         pose proof uvalue_convert_strict_safe f0.
+                         destruct H as (f0'&CONV1&CONV2).
+                         setoid_rewrite CONV1.
+                         rewrite F.
+                     - eapply IHRUN; eauto.
+                   }
+                 * specialize (EQ t1). contradiction.
+               + 
+
+               genobs m1 om1.
+               clear m1 Heqom1 IHRUN.
+
+               cbn in *.
+               
+
+               
+               repeat red in EV_REL.
+
+               
+                 assert (get_inf_tree {| _observe := t2 |} ≈ get_inf_tree (vis (@resum (Type -> Type) IFun OOME
+              (PickUvalueE +' OOME +' UBE +' DebugE +' FailureE)
+              (@ReSum_inr (Type -> Type) IFun sum1 Cat_IFun Inr_sum1 OOME
+                 (OOME +' UBE +' DebugE +' FailureE) PickUvalueE
+                 (@ReSum_inl (Type -> Type) IFun sum1 Cat_IFun Inl_sum1 OOME OOME
+                    (UBE +' DebugE +' FailureE)
+                    (@ReSum_id (Type -> Type) IFun Id_IFun OOME))) A o) (fun x : A => ITree.bind (ret (s2, (s1, x))) k2))).
+                 { 
+                   rewrite H1.
+                   reflexivity.
+                 }
+                 rewrite H2.
+                 eapply get_inf_tree_Proper.
+                 setoid_rewrite H1.
+               }
+               punfold H; red in H; cbn in H.
+               genobs m1 om1.
+               setoid_rewrite (itree_eta_ m1) in IHRUN.
+               rewrite <- Heqom1 in IHRUN.
+               clear m1 Heqom1.
+               dependent induction H.
+               + repeat red in H2.
+                 break_match_hyp.
+                 * red in H2.
+                   setoid_rewrite bind_trigger in H2.
+                   rewrite H2 in H3.
+                   setoid_rewrite bind_vis in H3.
+                   setoid_rewrite bind_ret_l in H3.
+                   inv Heqs.
+                   repeat red in H.
+                   destruct e1; try discriminate.
+                   2: { destruct s. destruct i; try contradiction.
+                        repeat destruct s; try contradiction.
+                   }
+                   destruct e, e0.
+                   destruct H as (?&?&?); subst.
+                   eapply Interp_Memory_PropT_Vis.
+                   2: {
+                     repeat red.
+                     setoid_rewrite bind_trigger.
+                     apply paco2_eqit_refl.
+                   }
+                   2: {
+                     rewrite H3.
+                     rewrite get_inf_tree_equation.
+                     cbn.
+                     rewrite <- bind_ret_r.
+                     eapply eutt_clo_bind. he
+
+H5 : DVCInfFin.uvalue_refine_strict f f0
+
+                     eapply eutt_clo_bind with
+                       (UU:=fun '(ms, (sid, ((lenv, stack), (genv, dv)))) '(ms', (sid', dv')) => ms = ms' /\ sid = sid' /\ dv = dv').
+                     2: {
+                       intros u1 u2 H.
+                       destruct u1 as (ms & (sid' & ((lenv & stack) & (genv & dv)))).
+                       destruct u2 as (ms' & (sid'' & dv')).
+                       destruct H as (?&?&?). subst.
+
+                       k2 := (fun '(ms, (sid, dv)) => SemNotations.Ret5 genv (lenv, stack) sid ms dv)
+
+                       unfold SemNotations.Ret5.
+
+                     }
+                       (t2 := (observe (vis
+       (subevent E1.DV.dvalue
+          (E1.ExternalCall t0 (fin_to_inf_uvalue f0) (map fin_to_inf_dvalue args0)))
+       (fun x0 : E1.DV.dvalue =>
+        get_inf_tree
+          match DVCInfFin.dvalue_convert_strict x0 with
+          | NoOom a => k2 (s2, (s1, a))
+          | Oom s => raiseOOM s
+          end)))).
+                     - pstep; red; cbn.
+                       constructor.
+                     reflexivity.
+
+                     
+
+  Notation res_L6 := (MemState * (store_id * (local_env * lstack * (global_env * dvalue))))%type.
+
+with (ta:=(vis (E1.ExternalCall t0 (fin_to_inf_uvalue f0) (map fin_to_inf_dvalue args0))
+       (fun x0 : E1.DV.dvalue =>
+        get_inf_tree
+          match DVCInfFin.dvalue_convert_strict x0 with
+          | NoOom a => k2 (s2, (s1, a))
+          | Oom s => raiseOOM s
+          end))).
+
+                     vis (E1.ExternalCall t0 (fin_to_inf_uvalue f0) (map fin_to_inf_dvalue args0))
+                       (fun x0 : E1.DV.dvalue =>
+                          get_inf_tree
+                            match DVCInfFin.dvalue_convert_strict x0 with
+                            | NoOom a => k2 (s2, (s1, a))
+                            | Oom s => raiseOOM s
+                            end)
+                     pstep; red; cbn.
+                     constructor.
+                     intros v.
+                     red.
+                     left.
+                     cbn.
+                     break_match.
+                     admit.
+                     - cbn.
+                     pose proof (dvalue_convert_strict_safe ).
+                     reflexivity.
+                     cbn.
+                   }
+                   -- intros a b H H7 H8.
+                      destruct b as (?&?&?); cbn in *; subst.
+                      pclearbot.
+                      left.
+
+                      pstep; red; cbn.
+                      econstructor.
+                      reflexivity.
+                      eapply upaco2_mon_bot; eauto.
+                      eapply H0.
+                      eauto.
+                      specialize (H0 a).
+                      forward H0.
+
+  H0 : forall (a : A0) (b : A),
+       L2_res_refine_strict A0 A e1 a (inl1 e0) b ->
+       upaco2
+         (orutt_ L2_refine_strict L2_res_refine_strict
+            (local_refine_strict × stack_refine_strict
+             × (global_refine_strict × DVCInfFin.dvalue_refine_strict))) bot2 
+         (k0 a) (k1 b)
+
+
+                 
+             - pclearbot.
+               
+               do 4 red in H0.
+               break_match_hyp.
+               + red in H0.
+                 setoid_rewrite bind_trigger in H0.
+                 rewrite H0 in H1.
+                 setoid_rewrite bind_vis in H1.
+                 punfold H1; red in H1; cbn in H1.
+                 dependent induction H1.
+                 * destruct e0.
+                   rewrite get_inf_tree_equation.
+                   cbn.
+                   reflexivity.
+                   (* TODO: Why won't this evaluate? *)
+                   admit.
+                 * 
+               + red in H0. repeat red in H0.
+                 
+               cbn in H0.
              - (* TauL *)
                clear IHRUN.
                pclearbot.
